Finished Trie Bag Implementation.

src/Common/FMapExtensions.v
@@ -1099,6 +1099,232 @@ Module FMapExtensions_fun (E: DecidableType) (Import M: WSfun E).
     intros; eapply elements_in_iff'; eauto.
   Qed.
 
+  Definition KeyBasedPartitioningFunction BagType reference :=
+    fun key (_: BagType) => if E.eq_dec key reference then true else false.
+
+    Lemma KeyBasedPartitioningFunction_Proper :
+      forall BagType reference,
+        Proper (E.eq ==> eq ==> eq) (KeyBasedPartitioningFunction BagType reference).
+    Proof.
+      intros;
+      unfold KeyBasedPartitioningFunction, Proper, respectful; intros x y E_eq **; subst;
+      destruct (F.eq_dec x _), (F.eq_dec y _); rewrite E_eq in *; intuition.
+    Qed.
+
+    Lemma negb_KeyBasedPartitioningFunction_Proper :
+      forall BagType reference,
+        Proper (E.eq ==> eq ==> eq)
+               (fun k e => negb (KeyBasedPartitioningFunction BagType reference k e)).
+    Proof.
+      intros;
+      unfold KeyBasedPartitioningFunction, Proper, respectful; intros x y E_eq **; subst;
+      destruct (F.eq_dec x _), (F.eq_dec y _); rewrite E_eq in *; intuition.
+    Qed.
+
+    Lemma eq_dec_refl :
+      forall x,
+        (if E.eq_dec x x then true else false) = true.
+    Proof.
+      intros; destruct (E.eq_dec _ _); eauto using E.eq_refl.
+    Qed.
+
+    Lemma eq_dec_comm :
+      forall x y,
+        (if E.eq_dec x y then true else false) = (if E.eq_dec y x then true else false).
+    Proof.
+      intros; destruct (E.eq_dec x y), (E.eq_dec y x); intuition.
+    Qed.
+
+    Lemma KeyBasedPartitioningFunction_eq_true :
+      forall TValue k k' v,
+        E.eq k k' <->
+        KeyBasedPartitioningFunction TValue k k' v = true.
+    Proof.
+      intros; unfold KeyBasedPartitioningFunction; destruct (E.eq_dec _ _); intuition.
+    Qed.
+
+    Lemma KeyBasedPartitioningFunction_eq_false :
+      forall TValue k k' v,
+        ~ E.eq k k' <->
+        KeyBasedPartitioningFunction TValue k k' v = false.
+    Proof.
+      intros; unfold KeyBasedPartitioningFunction; destruct (E.eq_dec _ _); intuition.
+    Qed.
+
+    Lemma KeyBasedPartitioningFunction_refl :
+      forall TValue k k' v,
+        KeyBasedPartitioningFunction TValue k k' v = KeyBasedPartitioningFunction TValue k' k v.
+    Proof.
+      intros; unfold KeyBasedPartitioningFunction; rewrite eq_dec_comm; reflexivity.
+    Qed.
+
+    (* The value [v] mapped to by [k] is the unique value [k] maps to. *)
+    Lemma KeyBasedPartition_fst_singleton :
+      forall {TValue} k v (m: t TValue),
+        MapsTo k v m ->
+        Equal (fst (partition (KeyBasedPartitioningFunction TValue k) m)) (add k v (empty TValue)).
+    Proof.
+
+      intros.
+      symmetry.
+      unfold Equal; intro key.
+
+      destruct (E.eq_dec key k) as [ eq_k_proj | neq_k_proj ].
+
+      rewrite eq_k_proj;
+        rewrite add_eq_o by eauto;
+        symmetry; rewrite <- find_mapsto_iff;
+        rewrite partition_iff_1 with (f := KeyBasedPartitioningFunction TValue k) (m := m);
+        intuition (try rewrite <- KeyBasedPartitioningFunction_eq_true;
+                   eauto using E.eq_refl, KeyBasedPartitioningFunction_Proper).
+
+      rewrite add_neq_o by eauto.
+      rewrite empty_o.
+      destruct (find key _) eqn:eqfind';
+        [ exfalso | eauto ].
+      rewrite <- find_mapsto_iff in eqfind'.
+      rewrite partition_iff_1 with (f := KeyBasedPartitioningFunction TValue k) (m := m) in eqfind'.
+      destruct eqfind' as (maps_to & kvpf_true).
+      apply neq_k_proj.
+      erewrite KeyBasedPartitioningFunction_eq_true.
+      rewrite KeyBasedPartitioningFunction_refl.
+      eauto.
+      eauto using KeyBasedPartitioningFunction_Proper.
+      reflexivity.
+    Qed.
+    
+    Lemma KeyBasedPartition_fst_singleton_None :
+      forall {TValue} k (m: t TValue),
+        ~ In k m ->
+        Equal (fst (partition (KeyBasedPartitioningFunction TValue k) m)) (empty TValue).
+    Proof.
+
+      intros.
+      symmetry.
+      unfold Equal; intro key.
+      rewrite empty_o; symmetry.
+      rewrite <- not_find_in_iff; unfold not; intros.
+      apply H.
+      destruct H0 as [v H0]; exists v.
+      unfold partition in H0; simpl in H0.
+      apply filter_iff in H0; eauto.
+      intuition eauto.
+      unfold KeyBasedPartitioningFunction in H2;
+        find_if_inside; try discriminate.
+      rewrite <- e; eauto.
+      eapply KeyBasedPartitioningFunction_Proper.
+    Qed.
+
+    (* If [k'] maps to a value in the first half of a map partitioned on [k],
+       it is equivalent to [k]. *)
+    Lemma MapsTo_KeyBasedPartition_fst :
+      forall {TValue} k k' v (m: t TValue),
+        MapsTo k' v (fst (partition (KeyBasedPartitioningFunction TValue k) m)) ->
+        E.eq k k'.
+    Proof.
+      intros * maps_to.
+      rewrite partition_iff_1
+      with (f := KeyBasedPartitioningFunction TValue k) (m := m)
+        in maps_to; eauto using KeyBasedPartitioningFunction_Proper.
+      destruct maps_to as (_ & kbpf_true).
+      rewrite <- KeyBasedPartitioningFunction_eq_true in kbpf_true.
+      trivial.
+    Qed.
+
+    Lemma In_KeyBasedPartition_fst :
+      forall {TValue} k k' (m: t TValue),
+        In k' (fst (partition (KeyBasedPartitioningFunction TValue k) m)) ->
+        E.eq k k'.
+    Proof.
+      intros * in_singleton.
+      apply In_MapsTo in in_singleton.
+      destruct in_singleton as [ val (maps_to & _) ].
+      eapply MapsTo_KeyBasedPartition_fst; eauto.
+    Qed.
+
+    (* If [k'] maps to a value in the second half of a map partitioned on [k],
+       it is *not* equivalent to [k]. *)
+    Lemma MapsTo_KeyBasedPartition_snd :
+      forall {TValue} k k' v (m: t TValue),
+        MapsTo k' v (snd (partition (KeyBasedPartitioningFunction TValue k) m)) ->
+        ~ E.eq k k'.
+    Proof.
+      intros * maps_to.
+      rewrite partition_iff_2
+      with (f := KeyBasedPartitioningFunction TValue k) (m := m)
+        in maps_to; eauto using KeyBasedPartitioningFunction_Proper.
+      destruct maps_to as (_ & kbpf_false).
+      rewrite <- KeyBasedPartitioningFunction_eq_false in kbpf_false.
+      trivial.
+    Qed.
+
+    Lemma In_KeyBasedPartition_snd :
+      forall {TValue} k k' (m: t TValue),
+        In k' (snd (partition (KeyBasedPartitioningFunction TValue k) m)) ->
+        ~ E.eq k k'.
+    Proof.
+      intros * in_falses.
+      apply In_MapsTo in in_falses.
+      destruct in_falses as [ val ( maps_to' & _ ) ].
+      eapply MapsTo_KeyBasedPartition_snd; eauto.
+    Qed.
+
+    (* Paritioning a finite map [m] augmented with a key [k] over [k]
+       will produce a map containing just [k] and a map equivalent to [m]. *)
+    Lemma partition_after_KeyBasedPartition_and_add :
+      forall {TValue} k v' (m: t TValue),
+        Partition (add k v' m)
+                  (add k v' (fst (partition (KeyBasedPartitioningFunction TValue k) m)))
+                  (snd (partition (KeyBasedPartitioningFunction TValue k) m)).
+    Proof.
+      unfold Partition.
+      split.
+
+      {
+        unfold Disjoint.
+        intros key (in_modified & in_unmodified).
+        rewrite add_in_iff in in_modified.
+
+        assert (E.eq k key)
+          by (
+              destruct in_modified;
+              [ assumption | eapply In_KeyBasedPartition_fst; eauto ]
+            ); clear in_modified.
+
+        apply In_KeyBasedPartition_snd in in_unmodified.
+
+        intuition.
+      }
+
+      split; intros * maps_to'.
+      rewrite add_mapsto_iff in maps_to'.
+      destruct maps_to' as [ (keq & veq) | (kneq & maps_to') ]; subst.
+
+      left;
+        apply add_1; eauto.
+      right;
+        rewrite partition_iff_2
+        with (f := KeyBasedPartitioningFunction TValue k) (m := m)
+        by (eauto using KeyBasedPartitioningFunction_Proper);
+        rewrite <- KeyBasedPartitioningFunction_eq_false;
+        intuition.
+
+      destruct maps_to' as [ maps_to' | maps_to' ].
+
+      rewrite add_mapsto_iff in maps_to';
+        destruct maps_to' as [ (keq & veq) | (kneq & maps_to') ];
+        [ subst; apply add_1; assumption | ].
+
+      exfalso.
+      apply MapsTo_KeyBasedPartition_fst in maps_to'.
+      intuition.
+
+      pose proof maps_to'.
+      apply MapsTo_KeyBasedPartition_snd in maps_to'.
+      apply add_2;
+        [ assumption | eapply MapsTo_partition_snd; eauto using KeyBasedPartitioningFunction_Proper ].
+    Qed.
+
 
 End FMapExtensions_fun.
 
