src/QueryStructure/Implementation/DataStructures/Bags/TrieBags.v
@@ -1,0 +1,2384 @@
+Require Export ADTSynthesis.QueryStructure.Implementation.DataStructures.Bags.BagsInterface
+        ADTSynthesis.QueryStructure.Implementation.DataStructures.Bags.BagsProperties.
+Require Import
+        Coq.FSets.FMapInterface
+        Coq.FSets.FMapFacts
+        Coq.FSets.FMapAVL
+        ADTSynthesis.Common
+        ADTSynthesis.Common.List.ListFacts
+        ADTSynthesis.Common.List.FlattenList
+        ADTSynthesis.Common.SetEqProperties
+        ADTSynthesis.Common.FMapExtensions
+        ADTSynthesis.Common.List.PermutationFacts.
+
+Module TrieBag (X:OrderedType).
+
+  Module XMap := FMapAVL.Make X.
+  Module Import XMapFacts := WFacts_fun X XMap.
+  Module Import MoreXMapFacts := FMapExtensions_fun X XMap.
+
+  Section TrieBagDefinitions.
+
+    Definition SearchTerm := list X.t.
+
+    Context {BagType TItem SearchTermType UpdateTermType : Type}
+            (TBag : Bag BagType TItem SearchTermType UpdateTermType)
+            (RepInv : BagType -> Prop)
+            (ValidUpdate : UpdateTermType -> Prop)
+            (TBagCorrect : CorrectBag RepInv ValidUpdate TBag)
+            (projection: TItem -> SearchTerm).
+
+    Import XMap.Raw.
+    Import XMap.Raw.Proofs.
+
+    Definition Map := t.
+
+    Inductive Trie :=
+    | Node : BagType -> Map Trie -> Trie.
+
+    Definition TrieNode (trie : Trie) :=
+      match trie with
+        | Node bag tries => bag
+      end.
+
+    Definition SubTries (trie : Trie) :=
+      match trie with
+        | Node bag tries => tries
+      end.
+
+    (* Emptiness *)
+
+    Definition TrieBag_bempty := Node bempty (empty Trie).
+
+    Fixpoint IsPrefix (st st' : SearchTerm) :=
+      match st, st' with
+        | [ ], _ => true
+        | s :: st, s' :: st' => if X.eq_dec s s' then IsPrefix st st' else false
+        | _, _ => false
+      end.
+
+    Definition TrieBag_bfind_matcher
+               (key_searchterm: SearchTerm * SearchTermType) (item: TItem) :=
+      let (keys, search_term) := key_searchterm in
+      IsPrefix (projection item) keys && (bfind_matcher search_term item).
+
+    Definition XMapfold
+               (A : Type) (f : X.t -> Trie -> A -> A) :=
+      fix XMapfold (m : tree Trie) (a : A) {struct m} : A :=
+      match m with
+        | XMap.Raw.Leaf => a
+        | XMap.Raw.Node l x d r _ => XMapfold r (f x d (XMapfold l a))
+      end.
+
+    Lemma XMapfold_eq A f
+    : forall m acc,
+        @XMapfold A f m acc =
+        @XMap.Raw.fold _ A f m acc.
+    Proof.
+      unfold XMapfold, XMap.Raw.fold; simpl.
+      induction m; eauto.
+      intros; rewrite IHm1, IHm2; reflexivity.
+    Qed.
+
+    Fixpoint Trie_enumerate
+             (t : Trie)
+             {struct t}
+    : list BagType :=
+      match t with
+        | Node bag tries =>
+          XMapfold (fun _ tries bags =>
+                      Trie_enumerate tries ++ bags) tries [bag]
+      end.
+
+    Definition TrieBag_benumerate
+               (container: Trie)
+      := flatten (List.map benumerate (Trie_enumerate container)).
+
+    Fixpoint Trie_find
+             (trie : Trie)
+             (st : SearchTerm)
+    : list BagType :=
+      (TrieNode trie) :: match st with
+                           | nil => [ ]
+                           | key :: st' =>
+                             match find key (SubTries trie) with
+                               | Some subtrie => Trie_find subtrie st'
+                               | None => [ ]
+                             end
+                         end.
+
+    Definition TrieBag_bcount
+               (trie : Trie)
+               (key_searchterm: SearchTerm * SearchTermType)
+    : nat :=
+      match key_searchterm with
+        | (st, search_term) =>
+          fold_left plus (List.map (fun bag : BagType => bcount bag search_term)
+                                   (Trie_find trie st)) 0
+      end.
+
+    Definition TrieBag_bfind
+               (trie : Trie)
+               (key_searchterm: SearchTerm * SearchTermType)
+    : list TItem :=
+      match key_searchterm with
+        | (st, search_term) =>
+          flatten (List.map (fun bag : BagType => bfind bag search_term)
+                            (Trie_find trie st))
+      end.
+
+    Fixpoint Trie_add
+             (trie : Trie)
+             (st : SearchTerm)
+             (item : TItem) : Trie :=
+      match st with
+        | [ ] =>
+          Node (binsert (TrieNode trie) item) (SubTries trie)
+        | key :: st' =>
+          match find key (SubTries trie) with
+            | Some subtrie =>
+              Node (TrieNode trie)
+                   (add key (Trie_add subtrie st' item)
+                        (SubTries trie))
+            | None =>
+              Node (TrieNode trie)
+                   (add key (Trie_add TrieBag_bempty st' item)
+                        (SubTries trie))
+          end
+      end.
+
+    Definition TrieBag_binsert
+               (trie : Trie)
+               (item: TItem) : Trie :=
+      Trie_add trie (projection item) item.
+
+    Fixpoint Trie_delete
+             (trie : Trie)
+             (st : SearchTerm)
+             (search_term : SearchTermType)
+    : (list TItem) * Trie :=
+      match st with
+        | nil =>
+          let (deletedItems, bag') :=
+              bdelete (TrieNode trie) search_term in
+          (deletedItems, Node bag' (SubTries trie))
+        | key :: st' =>
+          let (deletedItems, bag') :=
+              bdelete (TrieNode trie) search_term in
+          match find key (SubTries trie) with
+            | Some subtrie =>
+              let (deletedSubItems, bag'') :=
+                  Trie_delete subtrie st' search_term in
+              (deletedItems ++ deletedSubItems,
+               Node bag' (add key bag'' (SubTries trie)))
+            | None =>
+              (deletedItems, Node bag' (SubTries trie))
+          end
+      end.
+
+    Definition TrieBag_bdelete
+               (trie : Trie)
+               (key_searchterm : SearchTerm * SearchTermType)
+    : (list TItem) * Trie :=
+      let (st, search_term) := key_searchterm in
+      Trie_delete trie st search_term.
+
+    Fixpoint Trie_update
+             (trie : Trie)
+             (st : SearchTerm)
+             (search_term : SearchTermType)
+             (updateTerm : UpdateTermType)
+    : (list TItem) * Trie :=
+      match st with
+        | nil =>
+          let (updatedItems, bag') :=
+              bupdate (TrieNode trie) search_term updateTerm in
+          (updatedItems, Node bag' (SubTries trie))
+        | key :: st' =>
+          let (updatedItems, bag') :=
+              bupdate (TrieNode trie) search_term updateTerm in
+          match find key (SubTries trie) with
+            | Some subtrie =>
+              let (updatedSubItems, bag'') :=
+                  Trie_update subtrie st' search_term updateTerm in
+              (updatedItems ++ updatedSubItems,
+               Node bag' (add key bag'' (SubTries trie)))
+            | None =>
+              (updatedItems, Node bag' (SubTries trie))
+          end
+      end.
+
+    Definition TrieBag_bupdate
+               (trie : Trie)
+               (key_searchterm : SearchTerm * SearchTermType)
+               (updateTerm : UpdateTermType)
+    : (list TItem) * Trie :=
+      let (st, search_term) := key_searchterm in
+      Trie_update trie st search_term updateTerm.
+
+    Definition WFMap := bst.
+
+    Definition Prefix (s s' : SearchTerm) :=
+      exists s'', eqlistA X.eq (s ++ s'') s'.
+
+    Lemma IsPrefix_iff_Prefix :
+      forall (s s' : SearchTerm),
+        IsPrefix s s' = true <-> Prefix s s'.
+    Proof.
+      unfold Prefix; split; revert s'; induction s; intros s' H.
+      - eexists s'; reflexivity.
+      - destruct s'; simpl in H.
+        + discriminate.
+        + find_if_inside; [subst | discriminate].
+          apply_in_hyp IHs; destruct_ex; eexists; subst; eauto.
+          simpl; econstructor; eauto.
+      - simpl; reflexivity.
+      - destruct s'; simpl in *; destruct H.
+        + inversion H.
+        + inversion H; subst; find_if_inside; intuition eauto.
+    Qed.
+
+    Inductive TrieOK : Trie -> SearchTerm -> Prop :=
+    | NodeSomeOK :
+        forall bag subtries st,
+          RepInv bag
+          -> bst subtries
+          -> (forall (item: TItem),
+                List.In item (benumerate bag) ->
+                eqlistA X.eq (projection item) st)
+          -> (forall k subtrie,
+                MapsTo k subtrie subtries
+                -> TrieOK subtrie (st ++ [k]))
+          -> TrieOK (Node bag subtries) st.
+
+    Lemma SubTrieMapBST
+    : forall bag subtries st,
+        TrieOK (Node bag subtries) st
+        -> bst subtries.
+    Proof.
+      inversion 1; eauto.
+    Qed.
+
+    Lemma SubTrieMapBST'
+    : forall trie st,
+        TrieOK trie st -> bst (SubTries trie).
+    Proof.
+      inversion 1; eauto.
+    Qed.
+
+    Hint Resolve SubTrieMapBST SubTrieMapBST'.
+
+    Lemma TrieNode_RepInv
+    : forall bag subtries st,
+        TrieOK (Node bag subtries) st
+        -> RepInv bag.
+    Proof.
+      inversion 1; eauto.
+    Qed.
+
+    Lemma TrieNode_RepInv'
+    : forall trie st,
+        TrieOK trie st -> RepInv (TrieNode trie).
+    Proof.
+      inversion 1; eauto.
+    Qed.
+
+    Hint Resolve TrieNode_RepInv TrieNode_RepInv'.
+
+    Lemma SubTrieOK
+    : forall trie k subtrie st,
+        TrieOK trie st
+        -> find k (SubTries trie) = Some subtrie
+        -> TrieOK subtrie (st ++ [k]).
+    Proof.
+      destruct trie; simpl.
+      induction m; simpl in *; intros.
+      - discriminate.
+      - inversion H; subst.
+        case_eq (X.compare k0 k); intros; rewrite H1 in H0.
+        + eapply IHm1; eauto.
+          econstructor; simpl in *; eauto.
+          inversion H4; subst; eauto.
+        + injections; simpl in *.
+          eapply (H7 k0 _); eauto.
+        + eapply IHm2; eauto.
+          econstructor; simpl in *; eauto.
+          inversion H4; subst; eauto.
+    Qed.
+
+    Hint Resolve SubTrieOK.
+
+    Definition TrieBagRepInv (trie : Trie) := TrieOK trie [ ].
+
+    Definition TrieBag_ValidUpdate (update_term : UpdateTermType) :=
+      ValidUpdate update_term /\
+      forall K item,
+        eqlistA X.eq (projection item) K
+        -> eqlistA X.eq (projection (bupdate_transform update_term item)) K.
+
+    Lemma Trie_Empty_RepInv :
+      TrieBagRepInv (TrieBag_bempty).
+    Proof.
+      unfold TrieBagRepInv; intros; econstructor; simpl in *.
+      apply bempty_RepInv.
+      econstructor.
+      intros; elimtype False; eapply benumerate_empty; eauto.
+      intros; elimtype False; eapply empty_1; eauto.
+    Qed.
+
+    Functional Scheme Trie_add_ind := Induction for Trie_add Sort Prop.
+    Functional Scheme Trie_delete_ind := Induction for Trie_delete Sort Prop.
+    Functional Scheme Trie_update_ind := Induction for Trie_update Sort Prop.
+    Functional Scheme Trie_find_ind := Induction for Trie_find Sort Prop.
+    Hint Resolve add_bst.
+    Hint Constructors eqlistA.
+
+    Lemma Trie_add_Preserves_TreeOK
+    : forall trie item st1 st2,
+        eqlistA X.eq (projection item) (st2 ++ st1)
+        -> TrieOK trie st2
+        -> TrieOK (Trie_add trie st1 item) st2.
+    Proof.
+      intros trie item st1; eapply Trie_add_ind; intros; subst.
+      - econstructor; inversion H0; subst; eauto.
+        + eapply binsert_RepInv; eauto.
+        + intros; rewrite binsert_enumerate in H5 by eauto.
+          simpl in *; intuition; subst.
+          rewrite H, app_nil_r; reflexivity.
+      - econstructor; inversion H1; subst; simpl; eauto.
+        intros; destruct (X.eq_dec k key0).
+        apply find_1 in H6; eauto.
+        pose proof (add_1 subtries (Trie_add subtrie st' item0) (X.eq_sym e)) as H7; apply find_1 in H7; eauto.
+        rewrite H6 in H7; injections; intros; subst.
+        eapply H; eauto.
+        rewrite <- app_assoc.
+        rewrite H0.
+        apply eqlistA_app;
+          repeat first [econstructor; eauto
+                       | try reflexivity ].
+        apply H5.
+        apply MapsTo_1 with (x := key0).
+        symmetry; eauto.
+        apply find_2; eassumption.
+        apply H5.
+        eapply add_3 in H6; eauto.
+      - econstructor; inversion H1; subst; simpl; eauto.
+        + intros; destruct (X.eq_dec k key0).
+          apply find_1 in H6; eauto.
+          pose proof (add_1 subtries (Trie_add TrieBag_bempty st' item0) (X.eq_sym e)) as H7; apply find_1 in H7; eauto.
+          rewrite H6 in H7; injections; intros; subst.
+          eapply H; eauto.
+          rewrite <- app_assoc.
+          rewrite H0.
+          apply eqlistA_app;
+            repeat first [econstructor; eauto
+                         | try reflexivity ].
+          unfold TrieBagRepInv; intros; econstructor; simpl in *.
+          apply bempty_RepInv.
+          econstructor.
+          intros; elimtype False; eapply benumerate_empty; eauto.
+          intros; elimtype False; eapply empty_1; eauto.
+          apply H5.
+          eapply add_3 in H6; eauto.
+    Qed.
+
+    Corollary TrieBag_binsert_Preserves_RepInv :
+      binsert_Preserves_RepInv TrieBagRepInv TrieBag_binsert.
+    Proof.
+      unfold binsert_Preserves_RepInv; intros.
+      eapply Trie_add_Preserves_TreeOK; simpl.
+      reflexivity.
+      apply containerCorrect.
+    Qed.
+
+    Lemma TrieBag_bdelete_Preserves_RepInv :
+      bdelete_Preserves_RepInv TrieBagRepInv TrieBag_bdelete.
+    Proof.
+      unfold bdelete_Preserves_RepInv, TrieBagRepInv;
+      intros trie search_term; remember []; clear Heql; revert l.
+      unfold TrieBag_bdelete.
+      destruct search_term.
+      eapply Trie_delete_ind; intros; subst.
+      - econstructor; inversion containerCorrect; subst; eauto.
+        + pose proof (bdelete_RepInv bag search_term) as e'; simpl in *;
+          rewrite e0 in e'; eapply e'.
+          inversion containerCorrect; eauto.
+        + intros; eapply H1.
+          destruct (bdelete_correct bag search_term); eauto.
+          simpl in *; rewrite e0 in *; simpl in *.
+          rewrite H4 in H3.
+          rewrite In_partition; eauto.
+      - econstructor; inversion containerCorrect; subst; eauto.
+        + pose proof (bdelete_RepInv bag search_term) as e'; simpl in *;
+          rewrite e0 in e'; eapply e'; eauto.
+        + intros; eapply H2.
+          destruct (bdelete_correct bag search_term); eauto.
+          simpl in *; rewrite e0 in *; simpl in *.
+          rewrite H5 in H4.
+          rewrite In_partition; eauto.
+        + intros; destruct (X.eq_dec k key0).
+          * apply find_1 in H4; eauto.
+            simpl in *.
+            pose proof (add_1 subtries bag'' (X.eq_sym e)) as H7; apply find_1 in H7; eauto.
+            rewrite H4 in H7; injections; intros; subst.
+            rewrite e2 in H; eapply H.
+            eapply H3.
+            apply MapsTo_1 with (x := key0).
+            symmetry; eauto.
+            apply find_2; eauto.
+          * apply H3.
+            eapply add_3; eauto.
+      - simpl; econstructor; inversion containerCorrect; subst; eauto.
+        + pose proof (bdelete_RepInv bag search_term) as e'; simpl in *;
+          rewrite e0 in e'; eapply e'.
+          inversion containerCorrect; eauto.
+        + intros; eapply H1.
+          destruct (bdelete_correct bag search_term); eauto.
+          simpl in *; rewrite e0 in *; simpl in *.
+          rewrite H4 in H3.
+          rewrite In_partition; eauto.
+    Qed.
+
+    Lemma ValidUpdate_TrieBag_ValidUpdate :
+      forall updateTerm,
+        TrieBag_ValidUpdate updateTerm
+        -> ValidUpdate updateTerm.
+    Proof.
+      inversion 1; subst; eauto.
+    Qed.
+
+    Hint Resolve ValidUpdate_TrieBag_ValidUpdate.
+
+    Lemma TrieBag_bupdate_Preserves_RepInv :
+      bupdate_Preserves_RepInv
+        TrieBagRepInv
+        TrieBag_ValidUpdate
+        TrieBag_bupdate.
+    Proof.
+      unfold bupdate_Preserves_RepInv, TrieBagRepInv;
+      intros trie search_term update_term; remember [];
+      clear Heql; revert l.
+      unfold TrieBag_bupdate.
+      destruct search_term.
+      eapply Trie_update_ind; intros; subst.
+      - econstructor; inversion containerCorrect; subst; eauto.
+        + pose proof (bupdate_RepInv bag search_term updateTerm) as e'; simpl in *;  rewrite e0 in e'; eapply e'; eauto.
+        + intros; destruct (bupdate_correct bag search_term updateTerm);
+          eauto.
+          simpl in *; rewrite e0 in *; simpl in *.
+          rewrite H4 in H3.
+          apply in_app_or in H3; intuition.
+          * eapply H1; erewrite In_partition; eauto.
+          * rewrite in_map_iff in H6; destruct_ex; intuition.
+            inversion valid_update; subst.
+            apply H8; apply H1; rewrite In_partition; eauto.
+      - econstructor; inversion containerCorrect; subst; eauto.
+        + pose proof (bupdate_RepInv bag search_term updateTerm) as e'; simpl in *;  rewrite e0 in e'; eapply e'; eauto.
+        + intros; destruct (bupdate_correct bag search_term updateTerm);
+          eauto.
+          simpl in *; rewrite e0 in *; simpl in *.
+          rewrite H5 in H4.
+          apply in_app_or in H4; intuition.
+          * eapply H2; erewrite In_partition; eauto.
+          * rewrite in_map_iff in H7; destruct_ex; intuition.
+            inversion valid_update; subst.
+            apply H9; apply H2; rewrite In_partition; eauto.
+        + intros; destruct (X.eq_dec k key0).
+          * apply find_1 in H4; eauto.
+            simpl in *.
+            pose proof (add_1 subtries bag'' (X.eq_sym e)) as H7; apply find_1 in H7; eauto.
+            rewrite H4 in H7; injections; intros; subst.
+            rewrite e2 in H; eapply H; eauto.
+            eapply H3.
+            apply MapsTo_1 with (x := key0).
+            symmetry; eauto.
+            apply find_2; eauto.
+          * apply H3.
+            eapply add_3; eauto.
+      - simpl; econstructor; inversion containerCorrect; subst; eauto.
+        + pose proof (bupdate_RepInv bag search_term updateTerm) as e'; simpl in *;  rewrite e0 in e'; eapply e'; eauto.
+        + intros; destruct (bupdate_correct bag search_term updateTerm);
+          eauto.
+          simpl in *; rewrite e0 in *; simpl in *.
+          rewrite H4 in H3.
+          apply in_app_or in H3; intuition.
+          * eapply H1; erewrite In_partition; eauto.
+          * rewrite in_map_iff in H6; destruct_ex; intuition.
+            inversion valid_update; subst.
+            apply H8; apply H1; rewrite In_partition; eauto.
+    Qed.
+
+    Lemma Permutation_app_fold_left
+    : forall l bags,
+        Permutation ((fold_left
+                        (fun (a : list BagType) (p : key * Trie) =>
+                           Trie_enumerate (snd p) ++ a) l
+                        bags))
+                    (bags ++
+                          (fold_left
+                             (fun (a : list BagType) (p : key * Trie) =>
+                                Trie_enumerate (snd p) ++ a) l
+                             [ ])).
+    Proof.
+      induction l; simpl; intros.
+      - rewrite app_nil_r; reflexivity.
+      - rewrite IHl, <- app_assoc,
+        Permutation_app_comm, <- app_assoc.
+        f_equiv.
+        rewrite Permutation_app_comm, <- IHl, app_nil_r; reflexivity.
+    Qed.
+
+    Lemma Permutation_benumerate_fold_left
+    : forall l bags,
+        Permutation (List.map benumerate
+                              (fold_left
+                                 (fun (a : list BagType) (p : key * Trie) =>
+                                    Trie_enumerate (snd p) ++ a) l
+                                 bags))
+                    ((List.map benumerate bags) ++
+                                                (List.map benumerate (fold_left
+                                                                        (fun (a : list BagType) (p : key * Trie) =>
+                                                                           Trie_enumerate (snd p) ++ a) l
+                                                                        [ ]))).
+    Proof.
+      intros; rewrite Permutation_app_fold_left, map_app; eauto.
+    Qed.
+
+    Lemma XMapfoldBst A :
+      forall f m (acc : A) (WFm : bst m),
+        XMapfold f m acc =
+        XMap.fold f (XMap.Bst WFm) acc.
+    Proof.
+      intros; rewrite XMapfold_eq; reflexivity.
+    Qed.
+
+    Ltac replaceXMapfold :=
+      match goal with
+          |- context [XMapfold ?f ?m ?acc] =>
+          let Bst_m := fresh in
+          assert (bst m) as Bst_m;
+            [ eauto | setoid_rewrite (XMapfoldBst f acc Bst_m)]
+      end.
+
+    Lemma XMapfindBst elt :
+      forall k (m : Map elt) (WFm : bst m),
+        find k m = XMap.find k (XMap.Bst WFm).
+    Proof.
+      reflexivity.
+    Qed.
+
+    Lemma Tries_enumerate_app_Proper
+    : Proper
+        (X.eq ==> eq ==> Permutation (A:=BagType) ==> Permutation (A:=BagType))
+        (fun (_ : X.t) (tries : Trie) (bags : list BagType) =>
+           Trie_enumerate tries ++ bags).
+    Proof.
+      unfold Proper, respectful; intros.
+      subst; rewrite H1; reflexivity.
+    Qed.
+
+    Lemma Tries_enumerate_app_transpose_neqkey
+    : transpose_neqkey (Permutation (A:=BagType))
+                       (fun (_ : X.t) (tries : Trie) (bags : list BagType) =>
+                          Trie_enumerate tries ++ bags).
+    Proof.
+      unfold transpose_neqkey; intros; rewrite Permutation_app_swap, <- app_assoc; f_equiv; apply Permutation_app_swap.
+    Qed.
+
+    Lemma benumerate_bempty_nil :
+      benumerate bempty = nil.
+      pose proof benumerate_empty; unfold BagEnumerateEmpty in *.
+      induction (benumerate bempty); eauto.
+      simpl in *; elimtype False; eapply H; eauto.
+    Qed.
+
+    Lemma Proper_KeyBasedPartitioningFunction
+    : forall key, Proper (X.eq ==> eq ==> eq) (KeyBasedPartitioningFunction Trie key).
+      unfold Proper, respectful; intros; subst.
+      unfold KeyBasedPartitioningFunction.
+      repeat find_if_inside; eauto.
+      rewrite H in e; intuition.
+    Qed.
+
+    Lemma TrieBag_BagEnumerateEmpty :
+      BagEnumerateEmpty TrieBag_benumerate TrieBag_bempty.
+    Proof.
+      intros;
+      unfold BagEnumerateEmpty, TrieBag_benumerate, flatten; simpl.
+      rewrite app_nil_r; apply benumerate_empty.
+    Qed.
+
+    Lemma Trie_find_TreeOK
+    : forall trie st2 st1,
+        TrieOK trie st1
+        -> forall bag,
+             List.In bag (Trie_find trie st2)
+             -> RepInv bag.
+    Proof.
+      intros trie st2; eapply Trie_find_ind; intros; subst.
+      - inversion H; subst; eauto.
+        simpl in H0; intuition eauto; subst; eauto.
+      - simpl in H1; intuition; subst.
+        + inversion H0; subst; eauto.
+        + eapply (H (st1 ++ [key0])); eauto.
+      - simpl in H0; intuition; subst; eauto.
+    Qed.
+
+    Lemma TrieBag_BagCountCorrect :
+      BagCountCorrect TrieBagRepInv TrieBag_bcount TrieBag_bfind .
+    Proof.
+      unfold TrieBagRepInv, TrieBag_bcount, TrieBag_bfind, BagCountCorrect.
+      simpl; intros; destruct search_term as [ key search_term ].
+      rewrite length_flatten.
+      rewrite !foldright_compose.
+      rewrite <- !fold_left_rev_right.
+      rewrite map_map.
+      generalize (Trie_find_TreeOK key containerCorrect).
+      remember 0 as n; clear Heqn; revert n.
+      induction (Trie_find container key); simpl; eauto.
+      intros.
+      intros; rewrite IHl by eauto.
+      rewrite fold_right_app; simpl.
+      rewrite bcount_correct by eauto.
+      rewrite !fold_left_rev_right; simpl.
+      clear; revert n; induction l; simpl; eauto with arith.
+      intros; rewrite IHl; f_equal; omega.
+    Qed.
+
+    Lemma Permutation_KeyBasedPartition
+    : forall key m bst_m b,
+        Permutation
+          (fold
+             (fun (_ : XMap.Raw.key) (trie : Trie) (a : list BagType) =>
+                Trie_enumerate trie ++ a) m b)
+          (XMap.fold
+             (fun (_ : XMap.key) (trie : Trie) (a : list BagType) =>
+                Trie_enumerate trie ++ a)
+             (fst
+                (partition (KeyBasedPartitioningFunction Trie key)
+                           {|
+                             XMap.this := m;
+                             XMap.is_bst := bst_m |}))
+             (XMap.fold
+                (fun (_ : XMap.key) (trie : Trie) (a : list BagType) =>
+                   Trie_enumerate trie ++ a)
+                (snd
+                   (partition (KeyBasedPartitioningFunction Trie key)
+                              {|
+                                XMap.this := m;
+                                XMap.is_bst :=  bst_m |}))
+                b)) .
+    Proof.
+      intros.
+      pose proof (partition_Partition_simple
+                    _
+                    (KeyBasedPartitioningFunction Trie key0)
+                    (KeyBasedPartitioningFunction_Proper _ _)
+                    (XMap.Bst bst_m)) as part.
+      erewrite Partition_fold with
+      (f := (fun (_ : key) (trie : Trie) (a : list BagType) =>
+               Trie_enumerate trie ++ a))
+        (m := {| XMap.this := m; XMap.is_bst := bst_m |} )
+        (i := b);
+        (eauto using part, Permutation_Equivalence, Tries_enumerate_app_Proper, Tries_enumerate_app_transpose_neqkey).
+    Qed.
+
+    Lemma In_fold_left_split' :
+      forall bag l acc,
+        List.In bag
+                (acc ++ fold_left
+                     (fun (a0 : list BagType) (p : key * Trie) =>
+                        Trie_enumerate (snd p) ++ a0) l
+                     [ ])
+        <-> List.In bag
+                    ((fold_left
+                        (fun (a0 : list BagType) (p : key * Trie) =>
+                           Trie_enumerate (snd p) ++ a0) l
+                        acc)).
+    Proof.
+      induction l; simpl; intros.
+      - rewrite app_nil_r in *; eauto.
+        reflexivity.
+      - rewrite <- IHl.
+        split; intros.
+        rewrite <- app_assoc; apply in_or_app.
+        apply in_app_or in H; intuition eauto.
+        right; apply in_or_app; eauto.
+        rewrite <- IHl in H0.
+        rewrite <- !app_assoc in H0.
+        apply in_app_or in H0; intuition.
+        apply in_app_or in H; intuition.
+        apply in_app_or in H0; intuition.
+        apply in_or_app; intuition.
+        right; rewrite <- IHl; intuition.
+        apply in_or_app; intuition.
+        rewrite <- IHl in H0.
+        apply in_app_or in H0; intuition.
+        right.
+        rewrite <- IHl.
+        apply in_or_app; auto.
+    Qed.
+
+    Corollary In_fold_left_split :
+      forall (k : X.t) t bag l acc,
+        List.In (k, bag)
+                (List.map (fun bag0 : BagType => (t, bag0))
+                          (acc ++ fold_left
+                               (fun (a0 : list BagType) (p : key * Trie) =>
+                                  Trie_enumerate (snd p) ++ a0) l
+                               [ ]))
+        <-> List.In (k, bag)
+                    (List.map (fun bag0 : BagType => (t, bag0))
+                              (fold_left
+                                 (fun (a0 : list BagType) (p : key * Trie) =>
+                                    Trie_enumerate (snd p) ++ a0) l
+                                 acc)).
+    Proof.
+      intros; rewrite !in_map_iff;
+      split; intros; destruct_ex; intuition;
+      eexists; split; eauto.
+      rewrite In_fold_left_split' in H1; eauto.
+      rewrite <- In_fold_left_split' in H1; eauto.
+    Qed.
+
+    Lemma In_fold_left_map_split' :
+      forall bag l acc,
+        List.In bag
+                (acc ++ fold_left
+                     (fun (a0 : list (key * BagType)) (p : key * Trie) =>
+                      List.map (fun bag0 : BagType => (fst p, bag0))
+                               (Trie_enumerate (snd p)) ++ a0)
+                     l
+                     [ ])
+        <-> List.In bag
+                    (fold_left
+                         (fun (a0 : list (key * BagType)) (p : key * Trie) =>
+                               List.map (fun bag0 : BagType => (fst p, bag0))
+                                        (Trie_enumerate (snd p)) ++ a0)
+                         l
+                         acc).
+    Proof.
+      induction l; simpl; intros.
+      - rewrite app_nil_r in *; eauto.
+        reflexivity.
+      - rewrite <- IHl.
+        split; intros.
+        rewrite <- app_assoc; apply in_or_app.
+        apply in_app_or in H; intuition eauto.
+        right; apply in_or_app; eauto.
+        rewrite <- IHl in H0.
+        rewrite <- !app_assoc in H0.
+        apply in_app_or in H0; intuition.
+        apply in_app_or in H; intuition.
+        apply in_app_or in H0; intuition.
+        apply in_or_app; intuition.
+        right; rewrite <- IHl; intuition.
+        apply in_or_app; intuition.
+        rewrite <- IHl in H0.
+        apply in_app_or in H0; intuition.
+        right.
+        rewrite <- IHl.
+        apply in_or_app; auto.
+    Qed.
+
+    Lemma Trie_add_Correct
+    : forall trie item st1 st2,
+        eqlistA X.eq (projection item) (st2 ++ st1)
+        -> TrieOK trie st2
+        -> Permutation
+             (TrieBag_benumerate (Trie_add trie st1 item))
+             (item :: TrieBag_benumerate trie).
+    Proof.
+      intros trie item st1; eapply Trie_add_ind; intros; subst.
+      - destruct trie0; simpl.
+        unfold TrieBag_benumerate; simpl.
+        rewrite !XMapfold_eq, !fold_1 by eauto.
+        rewrite Permutation_benumerate_fold_left.
+        simpl; rewrite binsert_enumerate; eauto.
+        simpl; constructor.
+        symmetry.
+        rewrite Permutation_benumerate_fold_left; simpl.
+        reflexivity.
+      - destruct trie0; simpl.
+        unfold TrieBag_benumerate; simpl.
+        replaceXMapfold.
+        replaceXMapfold.
+        unfold XMap.fold at 2.
+
+        rewrite Permutation_KeyBasedPartition with (key0 := key0)
+                                                     (bst_m := SubTrieMapBST H1).
+
+        pose proof (@partition_after_KeyBasedPartition_and_add
+                      _ key0 (Trie_add subtrie st' item0) (XMap.Bst (SubTrieMapBST H1)))
+          as part_add.
+
+        rewrite Partition_fold at 1;
+          (eauto using part_add, Permutation_Equivalence, Tries_enumerate_app_Proper, Tries_enumerate_app_transpose_neqkey).
+
+        apply find_2 in e0.
+
+        pose proof (KeyBasedPartition_fst_singleton key0 subtrie (XMap.Bst (SubTrieMapBST H1)) e0) as singleton.
+        pose proof (add_Equal_simple singleton key0 (Trie_add subtrie st' item0)) as singleton'.
+        rewrite (fold_Equal_simpl (eqA := @Permutation BagType) singleton')
+          by (eauto using Permutation_Equivalence, Tries_enumerate_app_Proper, Tries_enumerate_app_transpose_neqkey).
+        rewrite (fold_Equal_simpl (eqA := @Permutation BagType) singleton)
+          by (eauto using Permutation_Equivalence, Tries_enumerate_app_Proper, Tries_enumerate_app_transpose_neqkey).
+        rewrite (fold_Equal_simpl (multiple_adds _ _ _ _))
+          by (eauto using Permutation_Equivalence, Tries_enumerate_app_Proper, Tries_enumerate_app_transpose_neqkey).
+        rewrite !fold_add
+          by (eauto using Permutation_Equivalence, Tries_enumerate_app_Proper, Tries_enumerate_app_transpose_neqkey, empty_In).
+
+        rewrite fold_empty.
+        rewrite !map_app.
+        unfold TrieBag_benumerate in H.
+        rewrite !flatten_app, (H (st2 ++ [key0])); eauto.
+        rewrite <- app_assoc; simpl; eauto.
+        inversion H1; subst; eauto.
+      - destruct trie0; simpl.
+        unfold TrieBag_benumerate; simpl.
+        replaceXMapfold.
+        replaceXMapfold.
+
+        pose proof (@partition_after_KeyBasedPartition_and_add
+                      _ key0 (Trie_add TrieBag_bempty st' item0) (XMap.Bst (SubTrieMapBST H1)))
+          as part_add.
+
+        pose proof (partition_Partition_simple
+                      _
+                      (KeyBasedPartitioningFunction Trie key0)
+                      (KeyBasedPartitioningFunction_Proper _ _)
+                      (XMap.Bst (SubTrieMapBST H1))) as part.
+
+        rewrite Partition_fold at 1;
+          (eauto using part_add, Permutation_Equivalence, Tries_enumerate_app_Proper, Tries_enumerate_app_transpose_neqkey).
+        rewrite Partition_fold with (m := {| XMap.this := m; XMap.is_bst := H3 |} );
+          (eauto using part, Permutation_Equivalence, Tries_enumerate_app_Proper, Tries_enumerate_app_transpose_neqkey).
+        rewrite !fold_add;
+          eauto using Permutation_Equivalence, Tries_enumerate_app_Proper, Tries_enumerate_app_transpose_neqkey, empty_In.
+        rewrite map_app, flatten_app.
+        rewrite (H (st2 ++ [key0])); simpl.
+        unfold TrieBag_benumerate; simpl.
+        rewrite benumerate_bempty_nil; simpl.
+        reflexivity.
+        rewrite <- app_assoc; eauto.
+        econstructor; eauto using bempty_RepInv.
+        + rewrite benumerate_bempty_nil in *; simpl in *; intuition.
+        + intros; elimtype False; eapply empty_1; eauto.
+        + intro H4.
+          destruct H4.
+          apply (@partition_iff_1 _
+                                  (KeyBasedPartitioningFunction Trie key0)
+                                  (Proper_KeyBasedPartitioningFunction key0)
+                                  {| XMap.this := m; XMap.is_bst := SubTrieMapBST H1 |}
+                                  _
+                                  key0 x
+                                  (refl_equal _)) in H4; intuition.
+          apply find_1 in H5; eauto; simpl in *; congruence.
+    Qed.
+
+    Corollary TrieBag_BagInsertEnumerate :
+      BagInsertEnumerate TrieBagRepInv TrieBag_benumerate TrieBag_binsert.
+    Proof.
+      unfold BagInsertEnumerate; intros; eapply Trie_add_Correct; eauto.
+      simpl; reflexivity.
+    Qed.
+
+    Definition XMapfold_ind
+               (P : Trie -> list BagType -> SearchTerm -> Prop)
+               (f : forall trie st, P trie (Trie_enumerate trie) st)
+               (m : tree Trie) (is_bst : bst m) :
+      forall k trie st , MapsTo k trie m ->
+                         P trie (Trie_enumerate trie) (st ++ [k]).
+      refine ((fix XMapfold (m : tree Trie) {struct m} :
+                 bst m ->
+                 forall k trie st, MapsTo k trie m ->
+                                   P trie (Trie_enumerate trie) (st ++ [k]) :=
+                 match m with
+                   | XMap.Raw.Leaf => _
+                   | XMap.Raw.Node l x d r _ => _
+                 end) m is_bst).
+      - intros; apply find_1 in H0; simpl in H0;
+        [ discriminate | eauto ].
+      - intros; apply find_1 in H0; simpl in H0;
+        [ destruct (X.compare k x)
+        | eassumption ].
+        + apply find_2 in H0.
+          eapply (XMapfold0 l); eauto.
+          inversion H; subst; eauto.
+        + pose proof (f d (st ++ [k])).
+          injections; eassumption.
+        + apply find_2 in H0.
+          eapply (XMapfold0 r); eauto.
+          inversion H; subst; eauto.
+    Defined.
+
+    Fixpoint Trie_enumerate_ind
+             (P : Trie -> list BagType -> SearchTerm -> Prop)
+             (H : forall trie st,
+                    (bst (SubTries trie)
+                     -> forall (k : key) (trie' : Trie),
+                          MapsTo k trie' (SubTries trie) -> P trie' (Trie_enumerate trie') (st ++ [k])) -> P trie (Trie_enumerate trie) st)
+             (trie : Trie)
+             (st : SearchTerm)
+             {struct trie}
+    : P trie (Trie_enumerate trie) st.
+    Proof.
+      refine (match trie with
+                | Node bag tries => _
+              end).
+      pose proof (@XMapfold_ind P (Trie_enumerate_ind P H) tries).
+      clear Trie_enumerate_ind.
+      eauto.
+    Qed.
+
+    Lemma TrieBag_enumerateOK
+    : forall l st1 (bags : list (key * BagType)) k bag,
+        (forall (k : X.t) (subtrie : Trie),
+           InA (PX.eqke (elt:=Trie)) (k, subtrie) l ->
+           TrieOK subtrie (st1 ++ [k])) ->
+        (forall (k : key) (bag : BagType),
+           List.In (k, bag) bags ->
+           forall (item: TItem),
+              List.In item (benumerate bag) ->
+              Prefix (st1 ++ [k]) (projection item))
+        -> List.In (k, bag) (fold_left
+                          (fun (a : list (key * BagType)) (p : key * Trie) =>
+                             (List.map (fun bag => (fst p, bag)) (Trie_enumerate (snd p)) ++ a)) l bags)
+        -> forall (item: TItem),
+              List.In item (benumerate bag) ->
+              Prefix (st1 ++ [k]) (projection item).
+    Proof.
+      induction l; simpl; eauto.
+      - intros.
+        rewrite <- In_fold_left_map_split' in H1.
+        rewrite <- app_assoc in H1.
+        apply in_app_or in H1; intuition eauto.
+        destruct a as [k' t]; simpl in *.
+        assert (InA (PX.eqke (elt:=Trie)) (k', t) ((k', t) :: l)) 
+               by (econstructor; eauto).
+        generalize (H k' t H1).
+        assert (k = k')
+          by (revert H3; clear; induction (Trie_enumerate t);
+              simpl; intro; intuition; injections; eauto).
+        subst.
+        apply in_map with (f := snd) in H3; rewrite map_map, map_id in H3.
+        remember (st1 ++ [k']).
+        setoid_rewrite <- Heql0.
+        generalize bag H2 H3; clear.
+        eapply (fun P H => @Trie_enumerate_ind P H t l0).
+        simpl; intros.
+        destruct trie; simpl in *.
+        rewrite !XMapfold_eq, !fold_1 in H3; eauto.
+        rewrite <- In_fold_left_split' in H3.
+        apply in_app_or in H3; intuition.
+        + simpl in H1; intuition; injections; subst.
+          inversion H0; subst.
+          apply H6 in H2; revert H2; clear.
+          * revert st; induction (projection item); simpl.
+            intros; inversion H2; subst.
+            eexists nil; rewrite app_nil_r.
+            constructor; symmetry; eauto.
+            eexists nil; simpl; rewrite app_nil_r; symmetry; eauto.
+        +  assert
+             (forall (k : key) (trie' : Trie),
+                InA (XMap.eq_key_elt (elt:=Trie)) (k,trie') (elements m) ->     List.In item (benumerate bag) ->
+                List.In (t, bag)
+                        (List.map (fun bag0 : BagType => (t, bag0)) (Trie_enumerate trie')) ->
+                TrieOK trie' (st ++ [k]) -> Prefix (st ++ [k]) (projection item)).
+           { intros; eapply H; eauto.
+             eapply (@XMap.elements_2 _ (XMap.Bst (SubTrieMapBST H0))); eauto.
+             apply in_map with (f := snd) in H5;
+               rewrite map_map, map_id in H5; simpl in *;
+               eauto.
+           }
+           assert (forall k' trie,
+                     InA (XMap.eq_key_elt (elt:=Trie)) (k', trie) (elements m)
+                     -> TrieOK trie (st ++ [k'])).
+           {  revert H0; clear.
+              intros; inversion H0; subst.
+              apply (@XMap.elements_2 _ (XMap.Bst H4)) in H.
+              apply H7 in H; simpl in H; eauto.
+           }
+           generalize st bag item b t H2 H3 H1 H4; clear.
+           induction (elements m); simpl; intros.
+           * intuition.
+           * rewrite <- In_fold_left_split' in H1.
+             apply in_app_or in H1; intuition eauto.
+             assert (forall a b c, Prefix (a ++ [b]) c ->
+                                   Prefix a c).
+             {
+               clear; intros; destruct H.
+               exists (b :: x); rewrite <- app_assoc in H; eauto.
+             }
+             destruct a; eapply H0; eapply H3.
+             econstructor; reflexivity.
+             eauto.
+             rewrite app_nil_r in H.
+             eauto.
+             simpl in H.
+             apply in_map_iff; eauto.
+             eapply H4; econstructor; eauto.
+             reflexivity.
+             eapply IHl; eauto.
+        + eapply IHl; eauto.
+          apply In_fold_left_map_split'; eauto.
+    Qed. 
+
+    Lemma TrieBag_enumerateOK1
+    : forall l st1 search_term bags,
+        (forall (k : X.t) (subtrie : Trie),
+           InA (PX.eqke (elt:=Trie)) (k, subtrie) l ->
+           TrieOK subtrie (st1 ++ [k])) ->
+        (forall (k : X.t) (bag : BagType) item,
+           List.In (k, bag) bags
+           -> List.In item (benumerate (Bag := TBag) bag)
+           -> Prefix (st1 ++ [k]) (projection item))
+        -> Permutation
+             (List.filter (TrieBag_bfind_matcher (st1, search_term))
+                          (flatten
+                             (List.map (fun p => benumerate (snd p))
+                                       (fold_left
+                                          (fun (a : list (key * BagType)) (p : key * Trie) =>
+                                             (List.map (fun bag => (fst p, bag)) (Trie_enumerate (snd p)) ++ a)) l bags))))
+             [].
+    Proof.
+      induction l; simpl; eauto.
+      - induction bags; simpl; intros; eauto.
+        rewrite filter_app, IHbags; eauto.
+        destruct a.
+        rewrite app_nil_r.
+        simpl.
+        generalize (fun item => H0 _ _ item (or_introl (refl_equal _))) ; clear; simpl.
+        induction (benumerate b); simpl; eauto.
+        intros.
+        case_eq (IsPrefix (projection a) st1); simpl; eauto.
+        find_if_inside; eauto.
+        intros.
+        pose proof (H _ (or_introl (refl_equal _))).
+        rewrite <- IsPrefix_iff_Prefix in H1.
+        elimtype False.
+        generalize st1 H0 H1; clear.
+        induction (projection a); simpl.
+        + destruct st1; simpl; congruence.
+        + destruct st1; simpl; try congruence.
+          repeat (find_if_inside; try congruence); eauto.
+      - intros; rewrite IHl; eauto.
+        intros.
+        apply in_app_or in H1; intuition eauto.
+        destruct a.
+        assert (InA (PX.eqke (elt:=Trie)) (t, t0) ((t, t0) :: l)) by
+            (econstructor; eauto).
+        apply H in H1; simpl in *.
+        assert (k = t).
+        {
+          revert H3; clear; induction (Trie_enumerate t0); simpl;
+          intros; intuition;  congruence.
+        }
+        subst.
+        revert H2 H3 H1.
+        clear.
+        eapply (fun P H => @Trie_enumerate_ind P H t0 (st1 ++ [t])).
+        simpl; intros.
+        destruct trie; simpl in *.
+        rewrite !XMapfold_eq, !fold_1 in H3; eauto.
+        rewrite <- In_fold_left_split, map_app in H3.
+        apply in_app_or in H3; intuition.
+        + simpl in H0; intuition; injections; subst.
+          inversion H1; subst.
+          apply H6 in H2; revert H2; clear.
+          * revert st; induction (projection item); simpl.
+            intros; inversion H2; subst.
+            eexists nil; rewrite app_nil_r.
+            constructor; symmetry; eauto.
+            eexists nil; simpl; rewrite app_nil_r; symmetry; eauto.
+        +  assert
+             (forall (k : key) (trie' : Trie),
+                InA (XMap.eq_key_elt (elt:=Trie)) (k,trie') (elements m) ->     List.In item (benumerate bag) ->
+                List.In (t, bag)
+                        (List.map (fun bag0 : BagType => (t, bag0)) (Trie_enumerate trie')) ->
+                TrieOK trie' (st ++ [k]) -> Prefix (st ++ [k]) (projection item)).
+           { intros; eapply H; eauto.
+             eapply (@XMap.elements_2 _ (XMap.Bst (SubTrieMapBST H1))); eauto. }
+           assert (forall k' trie,
+                     InA (XMap.eq_key_elt (elt:=Trie)) (k', trie) (elements m)
+                     -> TrieOK trie (st ++ [k'])).
+           {  revert H1; clear.
+              intros; inversion H1; subst.
+              apply (@XMap.elements_2 _ (XMap.Bst H4)) in H.
+              apply H7 in H; simpl in H; eauto.
+           }
+           generalize st bag item b t H2 H3 H0 H4; clear.
+           induction (elements m); simpl; intros.
+           * intuition.
+           * rewrite <- In_fold_left_split, map_app in H0.
+             apply in_app_or in H0; intuition eauto.
+             assert (forall a b c, Prefix (a ++ [b]) c ->
+                                   Prefix a c).
+             {
+               clear; intros; destruct H.
+               exists (b :: x); rewrite <- app_assoc in H; eauto.
+             }
+             destruct a; eapply H0; eapply H3.
+             econstructor; reflexivity.
+             eauto.
+             rewrite app_nil_r in H.
+             eauto.
+             eapply H4; econstructor; eauto.
+             reflexivity.
+             eapply IHl; eauto.
+    Qed.
+
+    Corollary TrieBag_enumerateOK'
+    : forall l st1 search_term,
+        (forall (k : X.t) (subtrie : Trie),
+           InA (PX.eqke (elt:=Trie)) (k, subtrie) l ->
+           TrieOK subtrie (st1 ++ [k]))
+        -> Permutation
+             (List.filter (TrieBag_bfind_matcher (st1, search_term))
+                          (flatten
+                             (List.map benumerate
+                                       (fold_left
+                                          (fun (a : list (BagType)) (p : key * Trie) =>
+                                             (Trie_enumerate (snd p)) ++ a) l [ ]))))
+             [].
+    Proof.
+      intros.
+      rewrite <- (@TrieBag_enumerateOK1 l st1 search_term [ ] H) by
+          intuition.
+      remember (@nil BagType); remember (@nil (X.t * BagType)).
+      assert (List.map snd l1 = l0) by (subst; eauto).
+      generalize l1 l0 H0; clear; induction l; simpl; intros.
+      rewrite <- map_map with (f := snd). setoid_rewrite H0.
+      reflexivity.
+      rewrite <- IHl; eauto.
+      rewrite map_app, map_map, map_id; simpl.
+      setoid_rewrite H0; reflexivity.
+    Qed.
+
+    Global Instance Prefix_refl :
+      Reflexive Prefix.
+    Proof.
+      intros; eexists nil; rewrite app_nil_r; reflexivity.
+    Qed.
+
+    Global Instance Prefix_trans :
+      Transitive Prefix.
+    Proof.
+      unfold Transitive;
+      intros; destruct H as [k H]; destruct H0 as [k' H0].
+      eexists (k ++ k'); rewrite <- H0, <- H, <- app_assoc; reflexivity.
+    Qed.
+
+    Add Parametric Relation
+    : (list _) (Prefix)
+        reflexivity proved by reflexivity
+        transitivity proved by transitivity
+          as refine_rel.
+
+    Lemma Prefix_app :
+      forall l l',
+        Prefix l (l ++ l').
+    Proof.
+      intros; eexists l'; reflexivity.
+    Qed.
+
+    Lemma filter_Prefix
+    : forall (b : BagType) m st l search_term',
+        TrieOK (Node b m) l
+        -> Prefix l st
+        -> Permutation (List.filter (bfind_matcher search_term') (benumerate b))
+                       (List.filter (TrieBag_bfind_matcher (st, search_term'))
+                                    (benumerate b)).
+    Proof.
+      intros; inversion H; subst.
+      revert H0 H5; clear.
+      induction (benumerate b); simpl; eauto.
+      intros; case_eq (IsPrefix (projection a) l); simpl; intros.
+      assert (IsPrefix (projection a) st = true) by
+          (rewrite IsPrefix_iff_Prefix in *; etransitivity; eauto).
+      rewrite H1; find_if_inside; simpl; rewrite IHl0; eauto.
+      assert (Prefix (projection a) l)
+        by (eexists nil; rewrite app_nil_r; eauto).
+      rewrite <- IsPrefix_iff_Prefix in H1; congruence.
+    Qed.
+
+    Lemma filter_negb_Prefix
+    : forall (b : BagType) m st l search_term',
+        TrieOK (Node b m) l
+        -> Prefix l st
+        -> Permutation (List.filter (fun a => negb (bfind_matcher search_term' a)) (benumerate b))
+                       (List.filter (fun a => negb (TrieBag_bfind_matcher (st, search_term') a))
+                                    (benumerate b)).
+    Proof.
+      intros; inversion H; subst.
+      revert H0 H5; clear.
+      induction (benumerate b); simpl; eauto.
+      intros; case_eq (IsPrefix (projection a) l); simpl; intros.
+      assert (IsPrefix (projection a) st = true) by
+          (rewrite IsPrefix_iff_Prefix in *; etransitivity; eauto).
+      rewrite H1; simpl; find_if_inside; simpl; rewrite IHl0; eauto.
+      assert (Prefix (projection a) l)
+        by (eexists nil; rewrite app_nil_r; eauto).
+      rewrite <- IsPrefix_iff_Prefix in H1; congruence.
+    Qed.
+
+    Lemma Prefix_cons_inv
+    : forall a l l',
+        Prefix (a :: l) (a :: l') -> Prefix l l'.
+    Proof.
+      induction l; simpl; intros.
+      - eexists l'; simpl; reflexivity.
+      - destruct H; inversion H; subst.
+        exists x; eauto.
+    Qed.
+
+    Lemma Prefix_app_inv
+    : forall a l l',
+        Prefix (a ++ l) (a ++ l') -> Prefix l l'.
+    Proof.
+      induction a; simpl; intros; eauto.
+      apply IHa; eapply Prefix_cons_inv; eauto.
+    Qed.
+
+    Lemma filter_remove_key :
+      forall key' m l st' search_term,
+        (forall (k : X.t) (subtrie : Trie),
+           InA (PX.eqke (elt:=Trie)) (k, subtrie)
+               (elements (remove key' (XMap.this m))) ->
+           TrieOK subtrie (l ++ [k]))
+        -> Permutation
+          (flatten
+             (List.map
+                (fun x : BagType =>
+                   List.filter
+                     (TrieBag_bfind_matcher (l ++ key' :: st', search_term))
+                     (benumerate x))
+                (XMap.fold
+                   (fun (_ : key) (trie : Trie) (a : list BagType) =>
+                      Trie_enumerate trie ++ a)
+                   (XMap.remove (elt:=Trie) key' m
+                   )
+                   []))) [].
+    Proof.
+      intros; unfold XMap.fold; rewrite fold_1; simpl; eauto.
+      remember (@nil BagType) as bags.
+      remember (@nil (key * BagType)) as bags'.
+      assert (forall (k0 : key) (bag0 : BagType),
+     List.In (k0, bag0) bags' ->
+     forall item : TItem,
+       List.In item (benumerate bag0) -> Prefix (l ++ [k0]) (projection item)) by (rewrite Heqbags'; intuition).
+      generalize
+           (fun k bag =>
+              @TrieBag_enumerateOK
+                (elements (remove key' (XMap.this m))) l bags' k bag
+                H H0).
+      clear H0.
+      assert (bags = List.map (@snd _ _) bags')  as H0
+        by (rewrite Heqbags', Heqbags; reflexivity);
+        rewrite H0; clear H0.
+      assert (forall (k : X.t) (subtrie : Trie),
+                InA (PX.eqke (elt:=Trie)) (k, subtrie)
+                    (elements (remove key' (XMap.this m))) ->
+                ~X.eq k key')
+        by (intros;
+            rewrite <- (@elements_mapsto_iff _ (XMap.Bst (remove_bst key' (XMap.is_bst m)))) in H0;
+            apply remove_mapsto_iff in H0; intuition).
+      assert (forall (k : X.t) b,
+                InA (PX.eqke (elt:=BagType)) (k, b) bags' ->
+                ~X.eq k key')
+        by (intros;
+            rewrite Heqbags' in *; inversion H1).
+      generalize bags' H H0 H1; clear; induction (elements (remove key' (XMap.this m))); simpl.
+      - induction bags'; simpl; intros; eauto.
+        rewrite IHbags'; eauto.
+        destruct a; simpl in *.
+        assert (~ X.eq k key') by
+            (intros; eapply H1; econstructor; eauto).
+        generalize (fun item => H2 k b (or_introl (refl_equal _)) item) H3;
+          clear.
+        induction (benumerate b); simpl; eauto; intros.
+        pose proof (H _ (or_introl (refl_equal _))).
+        rewrite <- IsPrefix_iff_Prefix in H0.
+        case_eq (IsPrefix (projection a) (l ++ key' :: st')); eauto.
+        intros.
+        rewrite IsPrefix_iff_Prefix in *.
+        assert (Prefix (l ++ [k]) (l ++ key' :: st')).
+        etransitivity; eauto.
+        pose proof (Prefix_app_inv _ _ _ H2).
+        destruct H4; inversion H4; subst.
+        elimtype False; eapply H3; eauto.
+      - intros.
+        rewrite <- (IHl0 ((List.map (fun a' => (fst a, a')) (Trie_enumerate (snd a))) ++ bags')); eauto.
+        rewrite map_app, map_map, map_id; reflexivity.
+        intros.
+        apply InA_app in H3; intuition eauto.
+        assert (~X.eq k (fst a))
+          by (destruct a; intro; eapply H0; eauto; econstructor).
+        apply H3; revert H5; clear; induction (Trie_enumerate (snd a));
+        intros; inversion H5; subst; eauto.
+        destruct H0; simpl in *; eauto.
+      - eapply (remove_bst _ (XMap.is_bst m)).
+    Qed.
+
+    Lemma elements_add_eq elt
+    : forall k (v : elt) m,
+        XMap.Equal (XMap.add k v m)
+                   (XMap.add k v (XMap.remove k m)).
+    Proof.
+      unfold XMap.Equal; intros.
+      symmetry; case_eq (XMap.find (elt:=elt) y (XMap.add k v m)); intros.
+      apply find_2 in H.
+      rewrite (@add_mapsto_iff _ m k y v e) in H; intuition; subst.
+      apply find_1; eauto.
+      exact (XMap.is_bst _).
+      apply add_1; eauto.
+      apply find_1; eauto.
+      exact (XMap.is_bst _).
+      apply add_2; eauto.
+      apply remove_2; eauto.
+      exact (XMap.is_bst _).
+      rewrite <- not_find_in_iff in *.
+      intro; apply H.
+      destruct H0.
+      rewrite (@add_mapsto_iff _ (XMap.remove k m) k y v x) in H0; intuition; subst.
+      eexists; eapply add_1; eauto.
+      rewrite (@remove_mapsto_iff _ m k y x) in H2; intuition.
+      eexists; eauto.
+      apply add_2; eauto.
+    Qed.
+
+    Lemma Permutation_benumerate_add
+    : forall k v m,
+        Permutation
+          (flatten
+             (List.map benumerate
+                       (fold_left
+                          (fun (a : list BagType) (p : XMap.key * Trie) =>
+                             Trie_enumerate (snd p) ++ a) (XMap.elements (XMap.add k v m))
+                          [])))
+          (flatten
+             (List.map benumerate
+                       (Trie_enumerate v ++
+                                       (fold_left
+                                          (fun (a : list BagType) (p : key * Trie) =>
+                                             Trie_enumerate (snd p) ++ a) (XMap.elements (XMap.remove k m))
+                                          [])))).
+    Proof.
+      intros; pose (@XMap.fold_1 _ (XMap.add k v m) _ nil
+                                 (fun _ (p : Trie) (a : list BagType) =>
+                                    Trie_enumerate p ++ a)).
+      simpl in e.
+      rewrite <- !e.
+      rewrite (fold_Equal_simpl (eqA := @Permutation BagType) (elements_add_eq k v m))
+        by (eauto using Permutation_Equivalence, Tries_enumerate_app_Proper, Tries_enumerate_app_transpose_neqkey).
+      rewrite !fold_add;
+        eauto using Permutation_Equivalence, Tries_enumerate_app_Proper, Tries_enumerate_app_transpose_neqkey, empty_In.
+      rewrite XMap.fold_1; simpl.
+      f_equiv.
+      eapply XMap.remove_1; reflexivity.
+    Qed.
+
+    Corollary TrieBag_enumerateOK'''
+    : forall l st1 key' st' search_term,
+        (forall (k : X.t) (subtrie : Trie),
+           InA (PX.eqke (elt:=Trie)) (k, subtrie) l ->
+           TrieOK subtrie (st1 ++ [k]))
+        -> ( forall (k : X.t) (subtrie : Trie),
+               InA (PX.eqke (elt:=Trie)) (k, subtrie)
+                   l -> ~X.eq k key')
+        -> Permutation
+             (List.filter (fun a => negb (TrieBag_bfind_matcher (st1 ++ key' :: st', search_term) a))
+                          (flatten
+                             (List.map benumerate
+                                       (fold_left
+                                          (fun (a : list (BagType)) (p : key * Trie) =>
+                                             (Trie_enumerate (snd p)) ++ a) l [ ]))))
+             (flatten
+                (List.map benumerate
+                          (fold_left
+                             (fun (a : list (BagType)) (p : key * Trie) =>
+                                (Trie_enumerate (snd p)) ++ a) l [ ]))).
+    Proof.
+      intros.
+      remember (@nil BagType) as bags.
+      remember (@nil (key * BagType)) as bags'.
+      assert (forall (k0 : key) (bag0 : BagType),
+                List.In (k0, bag0) bags' ->
+                forall item : TItem,
+                  List.In item (benumerate bag0) -> Prefix (st1 ++ [k0]) (projection item)) by (rewrite Heqbags'; intuition).
+      generalize
+        (fun k bag =>
+           @TrieBag_enumerateOK
+             l st1 bags' k bag
+             H H1).
+      clear H1.
+      assert (bags = List.map (@snd _ _) bags') as H1
+          by (rewrite Heqbags', Heqbags; reflexivity);
+        rewrite H1; clear H1.
+      assert (forall (k : X.t) b,
+                InA (PX.eqke (elt:=BagType)) (k, b) bags' ->
+                ~X.eq k key')
+        by (intros;
+            rewrite Heqbags' in *; inversion H1).
+      generalize bags' H H0 H1; clear; induction l; simpl; intros.
+      - induction bags'; simpl; intros; eauto.
+        rewrite filter_app, IHbags'; eauto; f_equiv.
+        destruct a; simpl in *.
+        assert (~ X.eq k key') by
+            (intros; eapply H1; econstructor; eauto).
+        generalize (fun item => H2 k b (or_introl (refl_equal _)) item) H3;
+          clear.
+        induction (benumerate b); simpl; eauto; intros.
+        pose proof (H _ (or_introl (refl_equal _))).
+        rewrite <- IsPrefix_iff_Prefix in H0.
+        case_eq (IsPrefix (projection a) (st1 ++ key' :: st')); eauto.
+        intros.
+        rewrite IsPrefix_iff_Prefix in *.
+        assert (Prefix (st1 ++ [k]) (st1 ++ key' :: st'))
+          by (etransitivity; eauto).
+        pose proof (Prefix_app_inv _ _ _ H2).
+        destruct H4; inversion H4; subst.
+        elimtype False; eapply H3; eauto.
+        simpl; intros; f_equiv.
+        generalize (fun item In_item => H item (or_intror In_item)).
+        generalize H3; clear; induction l; simpl; intros; eauto.
+        pose proof (H _ (or_introl (refl_equal _))).
+        case_eq (IsPrefix (projection a) (st1 ++ key' :: st')); eauto.
+        intros.
+        rewrite IsPrefix_iff_Prefix in *.
+        assert (Prefix (st1 ++ [k]) (st1 ++ key' :: st'))
+          by (etransitivity; eauto).
+        apply Prefix_app_inv in H2.
+        destruct H2; simpl in H2; inversion H2; subst.
+        intuition.
+        intros; simpl; rewrite IHl; eauto.
+        intros; eapply H2; eauto.
+        constructor 2; eauto.
+      - intros.
+        pose proof (IHl ((List.map (fun a' => (fst a, a')) (Trie_enumerate (snd a))) ++ bags')) as H'.
+        rewrite map_app, map_map, map_id in H'.
+        rewrite <- H' at 2; clear H'; intros.
+        rewrite !flatten_filter; eauto.
+        destruct a; eapply H; econstructor 2; eauto.
+        eapply H0; eauto.
+        apply InA_app in H3; intuition eauto.
+        assert (~X.eq k (fst a))
+          by (destruct a; intro; eapply H0; eauto; econstructor).
+        apply H3; revert H5; clear; induction (Trie_enumerate (snd a));
+        intros; inversion H5; subst; eauto.
+        destruct H0; simpl in *; eauto.
+        eapply H2; eauto.
+    Qed.
+
+    Lemma filter_negb_remove
+    : forall key m,
+        XMap.Equal (filter
+                      (fun (k : XMap.key) (e : Trie) =>
+                         negb (KeyBasedPartitioningFunction Trie key k e))
+                      m)
+                   (XMap.remove key m).
+    Proof.
+      unfold XMap.Equal; intros.
+      destruct (X.eq_dec key0 y).
+      - rewrite remove_eq_o; eauto.
+        rewrite <- e; unfold filter; clear y e.
+        destruct m; unfold XMap.fold; rewrite fold_1; simpl; eauto.
+        assert (XMap.find (elt:=Trie) key0 (XMap.empty Trie) = None).
+        { rewrite <- not_find_in_iff.
+          intro H; destruct H; simpl in *; eapply empty_1; eauto.
+        }
+        revert H.
+        remember (XMap.empty Trie); generalize t; clear Heqt.
+        induction (elements this); intros; simpl.
+        + eauto.
+        + eapply IHl.
+          case_eq (negb (KeyBasedPartitioningFunction Trie key0 (fst a) (snd a)));
+            intros; eauto.
+          rewrite add_neq_o; eauto.
+          intro; unfold KeyBasedPartitioningFunction in *.
+          case_eq (F.eq_dec (fst a) key0); intros; rewrite H2 in H0;
+          simpl in *; try congruence.
+      - rewrite remove_neq_o by eauto.
+        destruct m; unfold filter, XMap.fold; rewrite fold_1; simpl; eauto.
+        case_eq (XMap.find (elt:=Trie) y {| XMap.this := this; XMap.is_bst := is_bst |}).
+        + intros; apply find_2 in H.
+          pose (@elements_mapsto_iff _ (XMap.Bst is_bst)) as H2; simpl in H2;
+          unfold XMap.MapsTo in H2; simpl in H2; rewrite H2 in H;
+          unfold XMap.elements in H; simpl in H; clear H2.
+          assert (InA (XMap.eq_key_elt (elt:=Trie)) (y, t) (elements this) \/
+                  InA (XMap.eq_key_elt (elt:=Trie)) (y, t) (XMap.elements (XMap.empty Trie)))
+            by eauto.
+          assert (forall key' v, XMap.MapsTo key' v (XMap.empty Trie) ->
+                                 ~ X.eq key' key0)
+            by (unfold not; intros; eapply XMap.empty_1; eauto).
+          assert (forall key' v, XMap.MapsTo key' v (XMap.empty Trie) ->
+                                 ~ InA X.eq key' (List.map fst (elements this)))
+            by (unfold not; intros; eapply XMap.empty_1; eauto).
+          assert (forall key' v, InA X.eq key' (List.map fst (elements this))
+                                 -> ~ XMap.MapsTo key' v (XMap.empty Trie))
+            by (unfold not; intros; eapply XMap.empty_1; eauto).
+          assert (NoDupA X.eq (List.map fst (XMap.elements (elt:=_) (XMap.Bst is_bst)))).
+          { pose proof (@XMap.elements_3w _ (XMap.Bst is_bst)).
+            unfold XMap.eq_key, PX.eqk in H4.
+            revert H4; clear; induction (XMap.elements (XMap.Bst is_bst)); intros;
+            constructor; eauto;
+            inversion H4; subst;
+            [ | apply IHl; eauto].
+            intro; apply H1; revert H; clear; induction l; intros; inversion H; subst.
+            constructor; eauto.
+            constructor 2; eauto.
+          }
+          unfold XMap.elements in H4; simpl in H4.
+          revert H1 H0 H2 H3 H4.
+          remember (XMap.empty Trie) as t'; generalize t'; clear Heqt' H.
+          induction (elements this); intros; simpl.
+          destruct t'0; apply find_1; eauto.
+          apply elements_mapsto_iff; simpl in H0; intuition.
+          inversion H.
+          eapply IHl; simpl in *; intuition.
+          * unfold KeyBasedPartitioningFunction in *.
+            destruct (X.eq_dec (fst a) key0); simpl in *; eauto; try congruence.
+            destruct a; simpl in *.
+            eapply XMap.add_3 in H0; eauto.
+          * unfold KeyBasedPartitioningFunction in *.
+            destruct (X.eq_dec (fst a) key0); simpl in *; eauto; try congruence.
+            eapply XMap.add_3 in H0; eauto.
+          * inversion H; subst.
+            destruct H5; destruct a; simpl in *; subst.
+            right; rewrite <- elements_mapsto_iff; simpl.
+            unfold KeyBasedPartitioningFunction in *.
+            destruct (X.eq_dec k key0); simpl in *; eauto; try congruence.
+            rewrite e in H0; symmetry in H0; intuition.
+            apply add_1; eauto.
+            eauto.
+          * right; rewrite <- elements_mapsto_iff; simpl.
+            unfold KeyBasedPartitioningFunction in *.
+            destruct (X.eq_dec (fst a) key0); simpl in *; eauto; try congruence.
+            rewrite <- elements_mapsto_iff in *; simpl; eauto.
+            rewrite <- elements_mapsto_iff in *; simpl; eauto.
+            apply add_2; eauto.
+          * unfold KeyBasedPartitioningFunction in *.
+            destruct (F.eq_dec (fst a) key0); simpl in *; eauto.
+            pose proof (proj1 (add_mapsto_iff _ _ _ _ _) H0); intuition; subst.
+            inversion H4; subst; eauto.
+            rewrite H6 in H9; eauto.
+            eapply H3; eauto.
+          * unfold KeyBasedPartitioningFunction in *.
+            destruct (F.eq_dec (fst a) key0); simpl in *; eauto.
+            pose proof (proj1 (add_mapsto_iff _ _ _ _ _) H0); intuition; subst.
+            inversion H4; subst; eauto.
+            rewrite H6 in H9; eauto.
+            eapply H3; eauto.
+          *  unfold KeyBasedPartitioningFunction in *.
+             destruct (F.eq_dec (fst a) key0); simpl in *; eauto.
+             pose proof (proj1 (add_mapsto_iff _ _ _ _ _) H5); intuition; subst.
+             inversion H4; subst; eauto.
+             rewrite H6 in H9; eauto.
+             eapply H3; eauto.
+          * unfold KeyBasedPartitioningFunction in *.
+            destruct (F.eq_dec (fst a) key0); simpl in *; eauto.
+            pose proof (proj1 (add_mapsto_iff _ _ _ _ _) H5); intuition; subst.
+            inversion H4; subst; eauto.
+            rewrite H6 in H9; eauto.
+            eapply H3; eauto.
+          * inversion H4; eauto.
+          * inversion H4; eauto.
+        + intros; apply not_find_in_iff in H.
+          assert (forall v, ~ InA (XMap.eq_key_elt (elt:=Trie)) (y, v) (XMap.elements (XMap.Bst is_bst)) /\
+                            ~ InA (XMap.eq_key_elt (elt:=Trie)) (y, v) (XMap.elements (XMap.empty Trie))).
+          { unfold not in*; split; intros.
+            rewrite <- elements_mapsto_iff in H0.
+            apply H; eexists v; simpl in *; apply H0.
+            rewrite <- elements_mapsto_iff in H0.
+            eapply XMap.empty_1; eauto.
+          }
+          assert (forall key' v, XMap.MapsTo key' v (XMap.empty Trie) ->
+                                 ~ X.eq key' key0)
+            by (unfold not; intros; eapply XMap.empty_1; eauto).
+          assert (forall key' v, XMap.MapsTo key' v (XMap.empty Trie) ->
+                                 ~ InA X.eq key' (List.map fst (elements this)))
+            by (unfold not; intros; eapply XMap.empty_1; eauto).
+          assert (forall key' v, InA X.eq key' (List.map fst (elements this))
+                                 -> ~ XMap.MapsTo key' v (XMap.empty Trie))
+            by (unfold not; intros; eapply XMap.empty_1; eauto).
+          assert (NoDupA X.eq (List.map fst (XMap.elements (elt:=_) (XMap.Bst is_bst)))).
+          { pose proof (@XMap.elements_3w _ (XMap.Bst is_bst)).
+            unfold XMap.eq_key, PX.eqk in H4.
+            revert H4; clear; induction (XMap.elements (XMap.Bst is_bst)); intros;
+            constructor; eauto;
+            inversion H4; subst;
+            [ | apply IHl; eauto].
+            intro; apply H1; revert H; clear; induction l; intros; inversion H; subst.
+            constructor; eauto.
+            constructor 2; eauto.
+          }
+          unfold XMap.elements in H4; simpl in H4, H0.
+          unfold XMap.elements at 1 in H0; simpl in H0.
+          rewrite <- not_find_in_iff.
+          revert H1 H0 H2 H3 H4.
+          remember (XMap.empty Trie) as t'; generalize t'; clear Heqt' H.
+          induction (elements this); intros; simpl.
+          unfold not; intros; destruct H as [x H].
+          apply (proj2 (H0 x)).
+          rewrite <- elements_mapsto_iff; eassumption.
+          eapply IHl; simpl in *; intuition.
+          * unfold KeyBasedPartitioningFunction in *.
+            destruct (X.eq_dec (fst a) key0); simpl in *; eauto; try congruence.
+            destruct a; simpl in *.
+            eapply XMap.add_3 in H; eauto.
+          * apply (proj1 (H0 v)); eauto.
+          * unfold KeyBasedPartitioningFunction in *.
+            destruct (X.eq_dec (fst a) key0); simpl in *; eauto; try congruence.
+            apply (proj2 (H0 v)); eauto.
+            rewrite <- elements_mapsto_iff in H.
+            pose proof (proj1 (add_mapsto_iff _ _ _ _ _) H); intuition; subst.
+            apply (proj1 (H0 (snd a))); econstructor.
+            constructor; eauto.
+            apply (proj2 (H0 v)); rewrite <- elements_mapsto_iff; eauto.
+          * unfold KeyBasedPartitioningFunction in *.
+            destruct (X.eq_dec (fst a) key0); simpl in *; eauto; try congruence.
+            pose proof (proj1 (add_mapsto_iff _ _ _ _ _) H); intuition; subst.
+            inversion H4; subst; eauto.
+            rewrite H6 in H9; eauto.
+            eapply H2; eauto.
+          * unfold KeyBasedPartitioningFunction in *.
+            destruct (F.eq_dec (fst a) key0); simpl in *; eauto.
+            pose proof (proj1 (add_mapsto_iff _ _ _ _ _) H5); intuition; subst.
+            inversion H4; subst; eauto.
+            rewrite H6 in H9; eauto.
+            eapply H3; eauto.
+          * inversion H4; eauto.
+    Qed.
+
+    Hint Resolve filter_negb_Prefix filter_Prefix Prefix_app.
+
+    Lemma TrieOK_subtrie_remove
+    : forall b m l key' k subtrie,
+        TrieOK (Node b m) l
+        -> bst m
+        -> InA (PX.eqke (elt:=Trie)) (k, subtrie)
+            (elements
+               (remove key' m)) ->
+        TrieOK subtrie (l ++ [k]).
+    Proof.
+      intros.
+      inversion H; subst; intros; eapply H8.
+      assert (bst (remove key'
+                          (XMap.this
+                             {| XMap.this := m; XMap.is_bst := H0 |}))).
+      apply remove_bst; eauto.
+      rewrite <- (@elements_mapsto_iff _ (XMap.Bst H2)) in H1.
+      simpl in H1; unfold XMap.MapsTo in H1; simpl in H1.
+      eapply remove_3; eauto.
+    Qed.
+
+    Lemma TrieOK_subtrie_filter
+    : forall b m l bst_m f k subtrie,
+        Proper (X.eq ==> eq ==> eq) f
+        -> TrieOK (Node b m) l
+        -> InA (PX.eqke (elt:=Trie)) (k, subtrie)
+            (XMap.elements
+               (filter f
+                       {| XMap.this := m; XMap.is_bst := bst_m |})) ->
+        TrieOK subtrie (l ++ [k]).
+    Proof.
+      intros.
+      inversion H0; subst; intros; eapply H8.
+      rewrite <- elements_mapsto_iff in H1.
+      rewrite filter_iff in H1; intuition.
+    Qed.
+
+    Hint Resolve TrieOK_subtrie_remove TrieOK_subtrie_filter.
+
+    Lemma TrieBag_BagFindCorrect :
+      BagFindCorrect TrieBagRepInv TrieBag_bfind TrieBag_bfind_matcher TrieBag_benumerate.
+    Proof.
+      intros.
+      destruct search_term as (st, search_term).
+      unfold TrieBag_bfind.
+      rewrite <- (app_nil_l st) at 1.
+      unfold TrieBagRepInv; remember [] as l; clear Heql; revert l.
+      eapply Trie_find_ind; intros; subst; simpl.
+      - rewrite !app_nil_r, <- bfind_correct by eauto.
+        destruct trie; simpl.
+        unfold TrieBag_benumerate; simpl.
+        rewrite !XMapfold_eq, !fold_1 by eauto.
+        rewrite Permutation_benumerate_fold_left, flatten_app; simpl;
+        rewrite filter_app, app_nil_r; simpl.
+        rewrite <- app_nil_r; f_equiv.
+        + rewrite filter_Prefix; eauto; reflexivity.
+        + inversion H; subst.
+          eapply TrieBag_enumerateOK'; intros.
+          eapply H6.
+          eapply (@XMap.elements_2 _ (XMap.Bst (SubTrieMapBST' H))); eauto.
+      - rewrite <- H; eauto.
+        destruct trie; simpl in *.
+        unfold TrieBag_benumerate; simpl.
+        rewrite !XMapfold_eq, !fold_1 by eauto.
+        rewrite Permutation_benumerate_fold_left, flatten_app; simpl;
+        rewrite filter_app, app_nil_r; simpl; f_equiv.
+        rewrite <- bfind_correct by eauto.
+        + inversion H0; subst.
+          rewrite filter_Prefix; eauto.
+        + rewrite <- (fun H => @fold_1 _ m H (list BagType) [ ] (fun k trie a => Trie_enumerate trie ++ a)) by eauto.
+          rewrite Permutation_KeyBasedPartition with (key0 := key0)
+                                                       (bst_m := SubTrieMapBST H0).
+          simpl.
+          apply find_2 in e0.
+          pose proof (KeyBasedPartition_fst_singleton key0 subtrie (XMap.Bst (SubTrieMapBST H0)) e0) as singleton.
+          rewrite (fold_Equal_simpl (eqA := @Permutation BagType) singleton)
+            by (eauto using Permutation_Equivalence, Tries_enumerate_app_Proper, Tries_enumerate_app_transpose_neqkey).
+          rewrite !fold_add;
+            eauto using Permutation_Equivalence, Tries_enumerate_app_Proper, Tries_enumerate_app_transpose_neqkey, empty_In.
+          rewrite map_app, flatten_app, filter_app, <- app_nil_r.
+          f_equiv.
+          rewrite <- app_assoc; simpl; eauto.
+          rewrite fold_empty, flatten_filter,map_map.
+
+          rewrite (fold_Equal_simpl (eqA := @Permutation BagType) (filter_negb_remove key0 _))
+            by (eauto using Permutation_Equivalence, Tries_enumerate_app_Proper, Tries_enumerate_app_transpose_neqkey).
+          eapply filter_remove_key; eauto.
+      - rewrite !app_nil_r, <- bfind_correct by eauto.
+        destruct trie; simpl.
+        unfold TrieBag_benumerate; simpl.
+        rewrite !XMapfold_eq, !fold_1 by eauto.
+        rewrite Permutation_benumerate_fold_left, flatten_app; simpl;
+        rewrite filter_app, app_nil_r; simpl.
+        rewrite <- app_nil_r; f_equiv.
+        + rewrite filter_Prefix; eauto.
+        + rewrite <- (fun H => @fold_1 _ m H (list BagType) [ ] (fun k trie a => Trie_enumerate trie ++ a)) by eauto.
+          rewrite Permutation_KeyBasedPartition with (key0 := key0)
+                                                       (bst_m := SubTrieMapBST' H).
+          simpl in *.
+          rewrite <- (@not_find_in_iff _ (XMap.Bst (SubTrieMapBST' H)) key0) in e0.
+          pose proof (KeyBasedPartition_fst_singleton_None key0 (XMap.Bst (SubTrieMapBST H)) e0) as singleton.
+          rewrite (fold_Equal_simpl (eqA := @Permutation BagType) singleton)
+            by (eauto using Permutation_Equivalence, Tries_enumerate_app_Proper, Tries_enumerate_app_transpose_neqkey).
+          rewrite fold_empty, flatten_filter, map_map.
+          rewrite (fold_Equal_simpl (eqA := @Permutation BagType) (filter_negb_remove key0 _))
+            by (eauto using Permutation_Equivalence, Tries_enumerate_app_Proper, Tries_enumerate_app_transpose_neqkey).
+          eapply filter_remove_key; eauto.
+
+
+    Qed.
+
+    Corollary TrieBag_enumerateOK''
+    : forall l st1 search_term,
+        (forall (k : X.t) (subtrie : Trie),
+           InA (PX.eqke (elt:=Trie)) (k, subtrie) l ->
+           TrieOK subtrie (st1 ++ [k]))
+        -> Permutation
+             (List.filter (fun a => negb (TrieBag_bfind_matcher (st1, search_term) a))
+                          (flatten
+                             (List.map benumerate
+                                       (fold_left
+                                          (fun (a : list (BagType)) (p : key * Trie) =>
+                                             (Trie_enumerate (snd p)) ++ a) l [ ]))))
+             (flatten
+                (List.map benumerate
+                          (fold_left
+                             (fun (a : list (BagType)) (p : key * Trie) =>
+                                (Trie_enumerate (snd p)) ++ a) l [ ]))).
+    Proof.
+      intros; generalize (@TrieBag_enumerateOK' l st1 search_term H); clear.
+      induction (flatten
+                   (List.map benumerate
+                             (fold_left
+                                (fun (a : list (BagType)) (p : key * Trie) =>
+                                   (Trie_enumerate (snd p)) ++ a) l [ ])));
+        simpl; eauto.
+      find_if_inside; intros; simpl.
+      symmetry in H; apply Permutation_nil in H; discriminate.
+      eauto.
+    Qed.
+
+
+    Lemma TrieOK_distinct_subtries :
+      forall b m key' l k subtrie bst_m
+             (OK : TrieOK (Node b m) l),
+        InA (PX.eqke (elt:=Trie)) (k, subtrie)
+            (elements
+               (XMap.this
+                  (XMap.remove (elt:=Trie) key'
+                               {|
+                                 XMap.this := m;
+                                 XMap.is_bst := bst_m  |}))) ->
+        ~ X.eq k key'.
+    Proof.
+      simpl; intros.
+      assert (bst (remove key' m)) by eauto using remove_bst.
+      rewrite <- (@elements_mapsto_iff _ (XMap.Bst (H0))) in H;
+        simpl in H0.
+      unfold not; intros.
+      symmetry in H1; revert H1.
+      pose proof (@remove_mapsto_iff  _ (XMap.Bst (bst_m))).
+      eapply H1; simpl; eauto.
+    Qed.
+
+    Lemma TrieOK_distinct_subtries' :
+      forall b m key' l k subtrie bst_m
+             (OK : TrieOK (Node b m) l),
+        InA (PX.eqke (elt:=Trie)) (k, subtrie)
+            (elements
+               (XMap.this
+                  (filter
+                     (fun (k0 : XMap.key) (e : Trie) =>
+                        negb (KeyBasedPartitioningFunction Trie key' k0 e))
+                     {|
+                       XMap.this := m;
+                       XMap.is_bst := bst_m |}))) ->
+        ~ X.eq k key'.
+    Proof.
+      intros * OK H2.
+      assert (bst ((XMap.this
+                              (filter
+                                 (fun (k0 : XMap.key) (e : Trie) =>
+                                    negb (KeyBasedPartitioningFunction Trie key' k0 e))
+                                 {|
+                                   XMap.this := m;
+                                   XMap.is_bst := bst_m |})))) by exact (XMap.is_bst _).
+      intros; rewrite <- (@elements_mapsto_iff _ (XMap.Bst H) k subtrie) in H2.
+      apply (@filter_iff _ (fun (k0 : XMap.key) (e : Trie) =>
+                              negb
+                                (KeyBasedPartitioningFunction Trie key' k0 e))) in H2.
+      intuition.
+      unfold KeyBasedPartitioningFunction in *.
+      find_if_inside; simpl in *; try congruence.
+      unfold Proper, respectful; intros; subst.
+      unfold KeyBasedPartitioningFunction; repeat find_if_inside; eauto.
+      rewrite <- e in n; intuition.
+    Qed.
+
+    Lemma Proper_negb_KeyBasedPartitioningFunction
+    : forall key',
+        Proper (X.eq ==> eq ==> eq)
+               (fun (k0 : XMap.key) (e : Trie) =>
+                  negb (KeyBasedPartitioningFunction Trie key' k0 e)).
+    Proof.
+      unfold Proper, respectful, KeyBasedPartitioningFunction; intros.
+      repeat find_if_inside; subst; simpl; eauto.
+      rewrite H in n; intuition.
+    Qed.
+
+    Lemma TrieBag_BagDeleteCorrect :
+      BagDeleteCorrect TrieBagRepInv TrieBag_bfind TrieBag_bfind_matcher
+                       TrieBag_benumerate TrieBag_bdelete.
+    Proof.
+      destruct search_term as (st, search_term).
+      unfold TrieBag_bdelete.
+      split.
+      {
+        rewrite <- (app_nil_l st) at 2.
+        revert containerCorrect.
+        unfold TrieBagRepInv; remember [] as l; clear Heql; revert l.
+        eapply Trie_delete_ind; intros; subst; simpl.
+        - destruct (bdelete_correct (TrieNode trie) search_term0); eauto.
+          destruct trie; simpl.
+          unfold TrieBag_benumerate; simpl.
+          rewrite !XMapfold_eq, !fold_1 by eauto.
+          rewrite e0 in H.
+          rewrite partition_filter_neq.
+          rewrite Permutation_benumerate_fold_left, flatten_app; simpl.
+          rewrite (Permutation_benumerate_fold_left _ [b]), flatten_app; simpl.
+          rewrite filter_app.
+          rewrite H, partition_filter_neq, !app_nil_r; simpl.
+          f_equiv.
+          + eapply filter_negb_Prefix; eauto; reflexivity.
+          + inversion containerCorrect; subst.
+            rewrite <- TrieBag_enumerateOK'' at 1.
+            unfold TrieBag_bfind_matcher; reflexivity.
+            intros; eapply H7.
+            eapply (@XMap.elements_2 _ (XMap.Bst H4)); eauto.
+        - rewrite e2 in H; simpl in *.
+          destruct trie; simpl in *.
+          unfold TrieBag_benumerate; simpl.
+          rewrite !XMapfold_eq, !fold_1 by eauto.
+          rewrite partition_filter_neq.
+          rewrite Permutation_benumerate_fold_left, flatten_app; simpl.
+          rewrite (Permutation_benumerate_fold_left _ [b]), flatten_app; simpl.
+          rewrite !filter_app.
+          rewrite app_nil_r, <- app_assoc.
+          f_equiv.
+          + replace (bag') with (snd  (bdelete b search_term0))
+              by (rewrite e0; eauto).
+            destruct (bdelete_correct b search_term0); eauto.
+            rewrite H0.
+            rewrite partition_filter_neq.
+            eapply filter_negb_Prefix; eauto; reflexivity.
+          + simpl.
+            rewrite <- (fun H => @fold_1 _ m H (list BagType) [ ] (fun k trie a => Trie_enumerate trie ++ a)) by eauto.
+            rewrite Permutation_KeyBasedPartition with (key0 := key0)
+                                                         (bst_m := SubTrieMapBST containerCorrect).
+            simpl in *.
+            apply find_2 in e1.
+            pose proof (KeyBasedPartition_fst_singleton key0 subtrie (XMap.Bst (SubTrieMapBST containerCorrect)) e1) as singleton.
+            rewrite (fold_Equal_simpl (eqA := @Permutation BagType) singleton)
+              by (eauto using Permutation_Equivalence, Tries_enumerate_app_Proper, Tries_enumerate_app_transpose_neqkey).
+            rewrite !fold_add;
+              eauto using Permutation_Equivalence, Tries_enumerate_app_Proper, Tries_enumerate_app_transpose_neqkey, empty_In.
+            rewrite flatten_filter.
+            rewrite !map_app, fold_empty, !map_map.
+            rewrite flatten_app.
+            rewrite (Permutation_benumerate_add key0 bag'' (XMap.Bst (SubTrieMapBST containerCorrect))).
+            rewrite map_app, flatten_app.
+            f_equiv.
+            * rewrite (H (l ++ [key0])), partition_filter_neq.
+              unfold TrieBag_benumerate; rewrite flatten_filter, map_map.
+              unfold TrieBag_bfind_matcher; rewrite <- app_assoc.
+              repeat f_equiv.
+              inversion containerCorrect; subst; eauto.
+            * pose (@XMap.fold_1 _ (XMap.remove key0 (XMap.Bst (SubTrieMapBST containerCorrect)))
+                                 _ nil
+                                 (fun (_ : key) (trie : Trie) (a : list BagType) =>
+                                    Trie_enumerate trie ++ a)).
+              simpl in e;  unfold XMap.key, key in *; rewrite <- e.
+              rewrite (fold_Equal_simpl (eqA := @Permutation BagType) (filter_negb_remove key0 _))
+                by (eauto using Permutation_Equivalence, Tries_enumerate_app_Proper, Tries_enumerate_app_transpose_neqkey).
+              unfold XMap.fold.
+              rewrite !fold_1.
+              rewrite <- TrieBag_enumerateOK'''.
+              rewrite flatten_filter.
+              rewrite map_map.
+              unfold TrieBag_bfind_matcher.
+              f_equiv.
+              intros; eapply TrieOK_subtrie_remove; simpl in *;
+              eauto using Proper_negb_KeyBasedPartitioningFunction.
+              intros; eapply TrieOK_distinct_subtries; eauto.
+              exact (XMap.is_bst _).
+        - destruct trie; simpl in *.
+          unfold TrieBag_benumerate; simpl.
+          rewrite !XMapfold_eq, !fold_1 by eauto.
+          rewrite partition_filter_neq.
+          rewrite Permutation_benumerate_fold_left, flatten_app; simpl.
+          rewrite (Permutation_benumerate_fold_left _ [b]), flatten_app; simpl.
+          rewrite !filter_app.
+          rewrite app_nil_r, <- app_assoc.
+          f_equiv.
+          + replace (bag') with (snd  (bdelete b search_term0))
+              by (rewrite e0; eauto).
+            destruct (bdelete_correct b search_term0); eauto.
+            rewrite H.
+            rewrite partition_filter_neq.
+            eapply filter_negb_Prefix; eauto; reflexivity.
+          + simpl.
+            rewrite <- (fun H => @fold_1 _ m H (list BagType) [ ] (fun k trie a => Trie_enumerate trie ++ a)) by eauto.
+            rewrite Permutation_KeyBasedPartition with (key0 := key0)
+                                                         (bst_m := SubTrieMapBST containerCorrect).
+            simpl.
+            rewrite <- (@not_find_in_iff _ (XMap.Bst (SubTrieMapBST' containerCorrect)) key0) in e1.
+            pose proof (KeyBasedPartition_fst_singleton_None key0 (XMap.Bst (SubTrieMapBST containerCorrect)) e1) as singleton.
+            rewrite (fold_Equal_simpl (eqA := @Permutation BagType) singleton)
+              by (eauto using Permutation_Equivalence, Tries_enumerate_app_Proper, Tries_enumerate_app_transpose_neqkey).
+            rewrite !fold_empty;
+              eauto using Permutation_Equivalence, Tries_enumerate_app_Proper, Tries_enumerate_app_transpose_neqkey, empty_In.
+            unfold XMap.fold; rewrite !fold_1.
+            rewrite <- TrieBag_enumerateOK''' at 1.
+            unfold TrieBag_bfind_matcher.
+            f_equiv.
+            intros; eapply TrieOK_subtrie_filter; simpl in *;
+            eauto using Proper_negb_KeyBasedPartitioningFunction.
+            intros; eapply TrieOK_distinct_subtries'; eauto.
+            exact (XMap.is_bst _).
+      }
+      { rewrite <- (app_nil_l st) at 2.
+        revert containerCorrect.
+        unfold TrieBagRepInv; remember [] as l; clear Heql; revert l.
+        eapply Trie_delete_ind; intros; subst; simpl.
+        - destruct (bdelete_correct (TrieNode trie) search_term0); eauto.
+          destruct trie; simpl.
+          unfold TrieBag_benumerate; simpl.
+          rewrite !XMapfold_eq, !fold_1 by eauto.
+          rewrite e0 in H.
+          rewrite partition_filter_eq.
+          rewrite Permutation_benumerate_fold_left, flatten_app; simpl.
+          rewrite filter_app.
+          replace deletedItems with (fst (bdelete b search_term0)) by
+              (simpl in *; rewrite e0; eauto).
+          destruct (bdelete_correct b search_term0); eauto.
+          rewrite H2, partition_filter_eq; simpl.
+          rewrite <- app_nil_r at 1.
+          f_equiv.
+          + inversion containerCorrect; subst.
+            revert H7; clear.
+            induction (benumerate b); simpl; eauto.
+            intros; case_eq (IsPrefix (projection a) l); simpl; intros.
+            find_if_inside; simpl; rewrite IHl0; eauto.
+            rewrite app_nil_r, H; simpl; eauto.
+            rewrite andb_false_r; eauto.
+            find_if_inside.
+            simpl; rewrite app_nil_r, H; simpl.
+            assert (Prefix (projection a) l)
+              by (eexists nil; rewrite app_nil_r; eauto).
+            rewrite <- IsPrefix_iff_Prefix in H0; congruence.
+            assert (Prefix (projection a) l)
+              by (eexists nil; rewrite app_nil_r; eauto).
+            rewrite <- IsPrefix_iff_Prefix in H0; congruence.
+          + inversion containerCorrect; subst.
+            rewrite TrieBag_enumerateOK' at 1; eauto.
+            rewrite app_nil_r.
+            intros; eapply H9.
+            eapply (@XMap.elements_2 _ (XMap.Bst H6)); eauto.
+        - rewrite e2 in H; simpl in *.
+          destruct trie; simpl in *.
+          unfold TrieBag_benumerate; simpl.
+          rewrite !XMapfold_eq, !fold_1 by eauto.
+          rewrite partition_filter_eq.
+          rewrite Permutation_benumerate_fold_left, flatten_app; simpl.
+          rewrite !filter_app; simpl.
+          f_equiv.
+          + replace deletedItems with (fst (bdelete b search_term0))
+              by (rewrite e0; eauto).
+            destruct (bdelete_correct b search_term0); eauto.
+            rewrite H1, partition_filter_eq, app_nil_r.
+            inversion containerCorrect; subst.
+            intros; eapply filter_Prefix; eauto; reflexivity.
+          + rewrite (H (l ++ [key0])); simpl; eauto.
+            rewrite partition_filter_eq.
+            rewrite <- (fun H => @fold_1 _ m H (list BagType) [ ] (fun k trie a => Trie_enumerate trie ++ a)) by eauto.
+            rewrite Permutation_KeyBasedPartition with (key0 := key0)
+                                                         (bst_m := SubTrieMapBST containerCorrect).
+            simpl.
+            apply find_2 in e1.
+            pose proof (KeyBasedPartition_fst_singleton key0 subtrie (XMap.Bst (SubTrieMapBST containerCorrect)) e1) as singleton.
+            rewrite (fold_Equal_simpl (eqA := @Permutation BagType) singleton)
+              by (eauto using Permutation_Equivalence, Tries_enumerate_app_Proper, Tries_enumerate_app_transpose_neqkey).
+            rewrite !fold_add;
+              eauto using Permutation_Equivalence, Tries_enumerate_app_Proper, Tries_enumerate_app_transpose_neqkey, empty_In.
+            rewrite flatten_filter.
+            rewrite !map_app, fold_empty, !map_map.
+            rewrite flatten_app.
+            rewrite <- app_nil_r at 1.
+            f_equiv.
+            * unfold TrieBag_benumerate; rewrite flatten_filter, map_map, <- app_assoc; reflexivity.
+            * rewrite <- filter_remove_key; eauto.
+              rewrite (fold_Equal_simpl (eqA := @Permutation BagType) (filter_negb_remove key0 _))
+                by (eauto using Permutation_Equivalence, Tries_enumerate_app_Proper, Tries_enumerate_app_transpose_neqkey).
+              eauto.
+              simpl; eauto.
+        - destruct trie; simpl in *.
+          unfold TrieBag_benumerate; simpl.
+          rewrite !XMapfold_eq, !fold_1 by eauto.
+          rewrite partition_filter_eq.
+          rewrite Permutation_benumerate_fold_left, flatten_app; simpl.
+          rewrite !filter_app.
+          rewrite <- app_nil_r at 1.
+          f_equiv.
+          + replace deletedItems with (fst (bdelete b search_term0))
+              by (rewrite e0; eauto).
+            destruct (bdelete_correct b search_term0); eauto.
+            rewrite H0, partition_filter_eq, app_nil_r.
+            eapply filter_Prefix; eauto.
+          + simpl.
+            rewrite <- (fun H => @fold_1 _ m H (list BagType) [ ] (fun k trie a => Trie_enumerate trie ++ a)) by eauto.
+            rewrite Permutation_KeyBasedPartition with (key0 := key0)
+                                                         (bst_m := SubTrieMapBST containerCorrect).
+            rewrite <- (@not_find_in_iff _ (XMap.Bst (SubTrieMapBST' containerCorrect)) key0) in e1.
+            pose proof (KeyBasedPartition_fst_singleton_None key0 (XMap.Bst (SubTrieMapBST containerCorrect)) e1) as singleton.
+            rewrite (fold_Equal_simpl (eqA := @Permutation BagType) singleton)
+              by (eauto using Permutation_Equivalence, Tries_enumerate_app_Proper, Tries_enumerate_app_transpose_neqkey).
+            rewrite !fold_empty;
+              eauto using Permutation_Equivalence, Tries_enumerate_app_Proper, Tries_enumerate_app_transpose_neqkey, empty_In.
+            simpl.
+            rewrite (fold_Equal_simpl (eqA := @Permutation BagType) (filter_negb_remove key0 _))
+              by (eauto using Permutation_Equivalence, Tries_enumerate_app_Proper, Tries_enumerate_app_transpose_neqkey).
+            rewrite <- filter_remove_key, flatten_filter, map_map; eauto.
+      }
+    Qed.
+
+    Lemma TrieBag_BagUpdateCorrect :
+      BagUpdateCorrect TrieBagRepInv TrieBag_ValidUpdate
+                       TrieBag_bfind TrieBag_bfind_matcher
+                       TrieBag_benumerate bupdate_transform TrieBag_bupdate.
+    Proof.
+      destruct search_term as (st, search_term).
+      unfold TrieBag_bupdate.
+      split.
+      {
+        rewrite <- (app_nil_l st); rewrite app_nil_l at 1.
+        revert containerCorrect.
+        unfold TrieBagRepInv; remember [] as l; clear Heql; revert l valid_update.
+        eapply Trie_update_ind; intros; subst; simpl.
+        - destruct (bupdate_correct (TrieNode trie) search_term0 updateTerm); eauto.
+          destruct trie; simpl.
+          rewrite partition_filter_neq, partition_filter_eq.
+          unfold TrieBag_benumerate; simpl.
+          rewrite !XMapfold_eq, !fold_1 by eauto.
+          rewrite e0 in H, H0; simpl in *.
+          rewrite Permutation_benumerate_fold_left, flatten_app; simpl.
+          rewrite (Permutation_benumerate_fold_left _ [b]), flatten_app; simpl.
+          rewrite H, partition_filter_neq,
+          partition_filter_eq, !app_nil_r, !filter_app, <- !app_assoc ; simpl.
+          f_equiv.
+          + eapply filter_negb_Prefix; eauto; reflexivity.
+          + symmetry.
+            rewrite map_app, Permutation_app_swap, <- app_assoc; f_equiv.
+            f_equiv.
+            * symmetry; eapply filter_Prefix; eauto; reflexivity.
+            * inversion containerCorrect; subst.
+              rewrite TrieBag_enumerateOK'; simpl.
+              rewrite <- TrieBag_enumerateOK'' at 2.
+              unfold TrieBag_bfind_matcher; reflexivity.
+              intros; eapply H7; eapply (@elements_mapsto_iff _ (XMap.Bst H4)); eauto.
+              intros; eapply H7; eapply (@elements_mapsto_iff _ (XMap.Bst H4)); eauto.
+        - rewrite e2 in H; simpl in *.
+          destruct trie; simpl in *.
+          unfold TrieBag_benumerate; simpl.
+          rewrite !XMapfold_eq, !fold_1 by eauto.
+          rewrite partition_filter_neq, partition_filter_eq.
+          rewrite Permutation_benumerate_fold_left, flatten_app; simpl.
+          rewrite (Permutation_benumerate_fold_left _ [b]), flatten_app; simpl.
+          rewrite !filter_app.
+          rewrite app_nil_r, <- !app_assoc; simpl.
+          rewrite map_app.
+          replace (bag') with (snd  (bupdate b search_term0 updateTerm))
+            by (rewrite e0; eauto).
+          destruct (bupdate_correct b search_term0 updateTerm); eauto.
+          rewrite H0, partition_filter_neq, partition_filter_eq, <- !app_assoc.
+          f_equiv.
+          + eapply filter_negb_Prefix; eauto; reflexivity.
+          + symmetry; rewrite Permutation_app_swap, <- app_assoc.
+            f_equiv.
+            * symmetry; f_equiv; eapply filter_Prefix; eauto.
+            * rewrite <- (fun H => @fold_1 _ m H (list BagType) [ ] (fun k trie a => Trie_enumerate trie ++ a)) by eauto.
+              rewrite Permutation_KeyBasedPartition with (key0 := key0)
+                                                           (bst_m := SubTrieMapBST containerCorrect).
+              rewrite (Permutation_benumerate_add key0 bag'' (XMap.Bst (SubTrieMapBST containerCorrect))).
+              rewrite map_app, flatten_app.
+              rewrite (H (l ++ [key0])), partition_filter_neq, partition_filter_eq.
+              rewrite <- app_assoc.
+              symmetry; rewrite Permutation_app_swap; symmetry.
+              rewrite <- app_assoc.
+              f_equiv.
+              { simpl.
+                apply find_2 in e1.
+                pose proof (KeyBasedPartition_fst_singleton key0 subtrie (XMap.Bst (SubTrieMapBST containerCorrect)) e1) as singleton.
+                rewrite (fold_Equal_simpl (eqA := @Permutation BagType) singleton)
+                  by (eauto using Permutation_Equivalence, Tries_enumerate_app_Proper, Tries_enumerate_app_transpose_neqkey).
+                rewrite !fold_add;
+                  eauto using Permutation_Equivalence, Tries_enumerate_app_Proper, Tries_enumerate_app_transpose_neqkey, empty_In.
+                rewrite flatten_filter.
+                rewrite !map_app, fold_empty, !map_map.
+                rewrite flatten_app.
+                rewrite Permutation_app_swap, map_app.
+                rewrite (fold_Equal_simpl (eqA := @Permutation BagType) (filter_negb_remove key0 _))
+                    by (eauto using Permutation_Equivalence, Tries_enumerate_app_Proper, Tries_enumerate_app_transpose_neqkey).
+                rewrite filter_remove_key; eauto.
+                simpl.
+                unfold TrieBag_benumerate.
+                rewrite <- map_map.
+                rewrite flatten_filter, map_flatten.
+                setoid_rewrite map_id; setoid_rewrite map_id.
+                rewrite map_map, <- app_assoc; reflexivity.
+              }
+              simpl.
+              rewrite flatten_filter, map_map.
+              apply find_2 in e1.
+              pose proof (KeyBasedPartition_fst_singleton key0 subtrie (XMap.Bst (SubTrieMapBST containerCorrect)) e1) as singleton.
+              rewrite (fold_Equal_simpl (eqA := @Permutation BagType) singleton)
+                by (eauto using Permutation_Equivalence, Tries_enumerate_app_Proper, Tries_enumerate_app_transpose_neqkey).
+              rewrite !fold_add;
+                eauto using Permutation_Equivalence, Tries_enumerate_app_Proper, Tries_enumerate_app_transpose_neqkey, empty_In.
+              rewrite map_app, flatten_app.
+              symmetry; rewrite Permutation_app_swap; symmetry.
+              f_equiv.
+              { unfold TrieBag_benumerate;
+                rewrite <- map_map.
+                rewrite flatten_filter, <- app_assoc; simpl; reflexivity.
+              }
+              rewrite fold_empty.
+              rewrite (fold_Equal_simpl (eqA := @Permutation BagType) (filter_negb_remove key0 _))
+                by (eauto using Permutation_Equivalence, Tries_enumerate_app_Proper, Tries_enumerate_app_transpose_neqkey).
+              unfold XMap.fold, XMap.remove, XMap.elements; simpl.
+              rewrite fold_1; simpl.
+              rewrite <- TrieBag_enumerateOK'''; eauto.
+              rewrite flatten_filter, map_map; unfold TrieBag_bfind_matcher; reflexivity; eauto.
+              intros; eapply TrieOK_distinct_subtries; eauto.
+              apply remove_bst.
+              eauto.
+              eauto.
+              eauto.
+        - destruct trie; simpl in *.
+          unfold TrieBag_benumerate; simpl.
+          rewrite !XMapfold_eq, !fold_1 by eauto.
+          rewrite partition_filter_neq, partition_filter_eq.
+          rewrite Permutation_benumerate_fold_left, flatten_app; simpl.
+          rewrite (Permutation_benumerate_fold_left _ [b]), flatten_app; simpl.
+          rewrite !filter_app.
+          rewrite app_nil_r, <- !app_assoc; simpl.
+          rewrite map_app.
+          replace (bag') with (snd  (bupdate b search_term0 updateTerm))
+            by (rewrite e0; eauto).
+          destruct (bupdate_correct b search_term0 updateTerm); eauto.
+          rewrite H, partition_filter_neq, partition_filter_eq, <- !app_assoc.
+          f_equiv.
+          + eapply filter_negb_Prefix; eauto; reflexivity.
+          + symmetry; rewrite Permutation_app_swap, <- app_assoc.
+            f_equiv.
+            * rewrite filter_Prefix; eauto; reflexivity.
+            * simpl.
+              rewrite <- (fun H => @fold_1 _ m H (list BagType) [ ] (fun k trie a => Trie_enumerate trie ++ a)) by eauto.
+              rewrite Permutation_KeyBasedPartition with (key0 := key0)
+                                                           (bst_m := SubTrieMapBST containerCorrect).
+              simpl.
+              rewrite <- (@not_find_in_iff _ (XMap.Bst (SubTrieMapBST' containerCorrect)) key0) in e1.
+              pose proof (KeyBasedPartition_fst_singleton_None key0 (XMap.Bst (SubTrieMapBST containerCorrect)) e1) as singleton.
+              rewrite (fold_Equal_simpl (eqA := @Permutation BagType) singleton)
+                by (eauto using Permutation_Equivalence, Tries_enumerate_app_Proper, Tries_enumerate_app_transpose_neqkey).
+              rewrite !fold_empty;
+                eauto using Permutation_Equivalence, Tries_enumerate_app_Proper, Tries_enumerate_app_transpose_neqkey, empty_In.
+              rewrite <- app_nil_l; f_equiv.
+              {
+                replace (@nil TItem) with (List.map (bupdate_transform updateTerm) (@nil _)) by
+                    reflexivity.
+                f_equiv.
+                rewrite (fold_Equal_simpl (eqA := @Permutation BagType) (filter_negb_remove key0 _))
+                  by (eauto using Permutation_Equivalence, Tries_enumerate_app_Proper, Tries_enumerate_app_transpose_neqkey).
+                rewrite <- filter_remove_key; eauto.
+                rewrite flatten_filter, map_map; eauto.
+                eauto.
+              }
+              unfold XMap.fold; symmetry.
+              rewrite fold_1, <- TrieBag_enumerateOK''' at 1.
+              rewrite fold_1; unfold TrieBag_bfind_matcher; eauto.
+              exact (XMap.is_bst _).
+              eauto using Proper_negb_KeyBasedPartitioningFunction.
+              intros; eapply TrieOK_distinct_subtries'; eauto.
+              exact (XMap.is_bst _).
+      }
+      {
+        rewrite <- (app_nil_l st); rewrite app_nil_l at 1.
+        revert containerCorrect.
+        unfold TrieBagRepInv; remember [] as l; clear Heql; revert l valid_update.
+        eapply Trie_update_ind; intros; subst; simpl.
+        - destruct (bupdate_correct (TrieNode trie) search_term0 updateTerm); eauto.
+          destruct trie; simpl.
+          rewrite partition_filter_eq.
+          unfold TrieBag_benumerate; simpl.
+          rewrite !XMapfold_eq, !fold_1 by eauto.
+          rewrite e0 in H, H0; simpl in *.
+          rewrite Permutation_benumerate_fold_left, flatten_app; simpl.
+          rewrite H0, partition_filter_eq, !app_nil_r, !filter_app ; simpl.
+          rewrite <- app_nil_r at 1.
+          f_equiv.
+          + rewrite filter_Prefix; eauto; reflexivity.
+          + inversion containerCorrect; subst.
+            rewrite TrieBag_enumerateOK' at 1; eauto.
+            intros; eapply H7.
+            eapply (@XMap.elements_2 _ (XMap.Bst H4)); eauto.
+        - rewrite e2 in H; simpl in *.
+          destruct trie; simpl in *.
+          unfold TrieBag_benumerate; simpl.
+          rewrite !XMapfold_eq, !fold_1 by eauto.
+          rewrite partition_filter_eq.
+          rewrite Permutation_benumerate_fold_left, flatten_app; simpl.
+          rewrite !filter_app, app_nil_r; simpl.
+          replace (updatedItems) with (fst (bupdate b search_term0 updateTerm))
+            by (rewrite e0; eauto).
+          destruct (bupdate_correct b search_term0 updateTerm); eauto.
+          rewrite H1, partition_filter_eq.
+          f_equiv.
+          + rewrite filter_Prefix; eauto; reflexivity.
+          + rewrite (H (l ++ [key0])); simpl; eauto.
+            rewrite partition_filter_eq.
+            rewrite <- (fun H => @fold_1 _ m H (list BagType) [ ] (fun k trie a => Trie_enumerate trie ++ a)) by eauto.
+            rewrite Permutation_KeyBasedPartition with (key0 := key0)
+                                                         (bst_m := SubTrieMapBST containerCorrect).
+            simpl.
+            apply find_2 in e1.
+            pose proof (KeyBasedPartition_fst_singleton key0 subtrie (XMap.Bst (SubTrieMapBST containerCorrect)) e1) as singleton.
+            rewrite (fold_Equal_simpl (eqA := @Permutation BagType) singleton)
+              by (eauto using Permutation_Equivalence, Tries_enumerate_app_Proper, Tries_enumerate_app_transpose_neqkey).
+            rewrite !fold_add;
+              eauto using Permutation_Equivalence, Tries_enumerate_app_Proper, Tries_enumerate_app_transpose_neqkey, empty_In.
+            rewrite flatten_filter.
+            rewrite !map_app, fold_empty, !map_map.
+            rewrite flatten_app.
+            rewrite <- app_nil_r at 1.
+            f_equiv.
+            * unfold TrieBag_benumerate; rewrite flatten_filter, map_map, <- app_assoc; reflexivity.
+            * rewrite <- filter_remove_key; eauto.
+              rewrite (fold_Equal_simpl (eqA := @Permutation BagType) (filter_negb_remove key0 _))
+                by (eauto using Permutation_Equivalence, Tries_enumerate_app_Proper, Tries_enumerate_app_transpose_neqkey).
+              eauto.
+              eauto.
+        - destruct trie; simpl in *.
+          unfold TrieBag_benumerate; simpl.
+          rewrite !XMapfold_eq, !fold_1 by eauto.
+          rewrite partition_filter_eq.
+          rewrite Permutation_benumerate_fold_left, flatten_app; simpl.
+          rewrite !filter_app, app_nil_r; simpl.
+          replace (updatedItems) with (fst (bupdate b search_term0 updateTerm))
+            by (rewrite e0; eauto).
+          destruct (bupdate_correct b search_term0 updateTerm); eauto.
+          rewrite H0, partition_filter_eq.
+          rewrite <- app_nil_r at 1.
+          f_equiv.
+          + rewrite filter_Prefix; eauto.
+          + simpl.
+            rewrite <- (fun H => @fold_1 _ m H (list BagType) [ ] (fun k trie a => Trie_enumerate trie ++ a)) by eauto.
+            rewrite Permutation_KeyBasedPartition with (key0 := key0)
+                                                         (bst_m := SubTrieMapBST containerCorrect).
+            rewrite <- (@not_find_in_iff _ (XMap.Bst (SubTrieMapBST' containerCorrect)) key0) in e1.
+            pose proof (KeyBasedPartition_fst_singleton_None key0 (XMap.Bst (SubTrieMapBST containerCorrect)) e1) as singleton.
+            rewrite (fold_Equal_simpl (eqA := @Permutation BagType) singleton)
+              by (eauto using Permutation_Equivalence, Tries_enumerate_app_Proper, Tries_enumerate_app_transpose_neqkey).
+            rewrite !fold_empty;
+              eauto using Permutation_Equivalence, Tries_enumerate_app_Proper, Tries_enumerate_app_transpose_neqkey, empty_In.
+            simpl.
+            rewrite (fold_Equal_simpl (eqA := @Permutation BagType) (filter_negb_remove key0 _))
+              by (eauto using Permutation_Equivalence, Tries_enumerate_app_Proper, Tries_enumerate_app_transpose_neqkey).
+            rewrite <- filter_remove_key; eauto.
+            rewrite flatten_filter, map_map; eauto.
+            eauto.
+            Grab Existential Variables.
+            eauto.
+      }
+    Qed.
+
+  End TrieBagDefinitions.
+
+  Global Instance TrieAsBag
+         {BagType TItem SearchTermType UpdateTermType : Type}
+         (TBag : Bag BagType TItem SearchTermType UpdateTermType)
+         projection
+  : Bag Trie TItem ((list TKey) * (SearchTermType)) UpdateTermType :=
+    {|
+
+      bempty            := TrieBag_bempty TBag;
+
+      bfind_matcher     := TrieBag_bfind_matcher TBag projection;
+      bupdate_transform := bupdate_transform;
+
+      benumerate := TrieBag_benumerate TBag;
+      bfind      := TrieBag_bfind TBag;
+      binsert    := TrieBag_binsert TBag projection;
+      bcount     := TrieBag_bcount TBag;
+      bdelete    := TrieBag_bdelete TBag;
+      bupdate    := TrieBag_bupdate TBag |}.
+
+  Global Instance TrieBagAsCorrectBag
+         {BagType TItem SearchTermType UpdateTermType : Type}
+         (TBag : Bag BagType TItem SearchTermType UpdateTermType)
+         (RepInv : BagType -> Prop)
+         (ValidUpdate : UpdateTermType -> Prop)
+         (CorrectTBag : CorrectBag RepInv ValidUpdate TBag)
+         projection
+  : CorrectBag (TrieBagRepInv TBag RepInv projection)
+               (TrieBag_ValidUpdate _ ValidUpdate projection)
+               (TrieAsBag TBag projection ) :=
+    {|
+      bempty_RepInv     := Trie_Empty_RepInv CorrectTBag projection;
+      binsert_RepInv    := @TrieBag_binsert_Preserves_RepInv _ _ _ _ TBag _ _ _ projection;
+      bdelete_RepInv    := @TrieBag_bdelete_Preserves_RepInv _ _ _ _ TBag _ _ _ projection;
+      bupdate_RepInv    := @TrieBag_bupdate_Preserves_RepInv _ _ _ _ TBag _ _ CorrectTBag projection;
+
+      binsert_enumerate := @TrieBag_BagInsertEnumerate _ _ _ _ _ _ _ CorrectTBag projection;
+      benumerate_empty  := @TrieBag_BagEnumerateEmpty _ _ _ _ _ _ _ CorrectTBag;
+      bfind_correct     := @TrieBag_BagFindCorrect _ _ _ _ _ _ _ CorrectTBag projection;
+      bcount_correct    := @TrieBag_BagCountCorrect _ _ _ _ _ _ _ CorrectTBag projection;
+      bdelete_correct   := @TrieBag_BagDeleteCorrect _ _ _ _ _ _ _ CorrectTBag projection ;
+      bupdate_correct   := @TrieBag_BagUpdateCorrect _ _ _ _ _ _ _ CorrectTBag projection
+    |}.
+
+End TrieBag.
+
